Hashmap/DHashMap/Lemmas.lean
@@ -69,7 +69,7 @@ theorem isEmpty_emptyc : (∅ : Raw α β).isEmpty :=
   isEmpty_empty
 
 @[simp]
-theorem isEmpty_insert [EquivBEq α] [LawfulHashable α] {a : α} {b : β a} : (m.insert a b).isEmpty = false := by
+theorem isEmpty_insert [EquivBEq α] [LawfulHashable α] {k : α} {v : β k} : (m.insert k v).isEmpty = false := by
   dhashmap_simp_to_raw using Raw₀.isEmpty_insert
 
 theorem contains_congr [EquivBEq α] [LawfulHashable α] {a b : α} (hab : a == b) : m.contains a = m.contains b := by
@@ -91,27 +91,27 @@ theorem mem_congr [EquivBEq α] [LawfulHashable α] {a b : α} (hab : a == b) : 
   not_mem_empty
 
 @[simp]
-theorem contains_insert [EquivBEq α] [LawfulHashable α] {a k : α} {b : β a} : (m.insert a b).contains k = (a == k || m.contains k) := by
+theorem contains_insert [EquivBEq α] [LawfulHashable α] {a k : α} {v : β k} : (m.insert k v).contains a = (a == k || m.contains a) := by
   dhashmap_simp_to_raw using Raw₀.contains_insert
 
 @[simp]
-theorem mem_insert [EquivBEq α] [LawfulHashable α] {a k : α} {b : β a} : k ∈ m.insert a b ↔ a == k ∨ k ∈ m := by
+theorem mem_insert [EquivBEq α] [LawfulHashable α] {k a : α} {v : β k} : a ∈ m.insert k v ↔ a == k ∨ a ∈ m := by
   simp [mem_iff_contains, contains_insert h]
 
-theorem contains_of_contains_insert [EquivBEq α] [LawfulHashable α] {a k : α} {b : β a} :
-    (m.insert a b).contains k → (a == k) = false → m.contains k := by
+theorem contains_of_contains_insert [EquivBEq α] [LawfulHashable α] {a k : α} {v : β k} :
+    (m.insert k v).contains a → (a == k) = false → m.contains a := by
   dhashmap_simp_to_raw using Raw₀.contains_of_contains_insert
 
-theorem mem_of_mem_insert [EquivBEq α] [LawfulHashable α] {a k : α} {b : β a} :
-    k ∈ m.insert a b → (a == k) = false → k ∈ m := by
+theorem mem_of_mem_insert [EquivBEq α] [LawfulHashable α] {k a : α} {v : β k} :
+    a ∈ m.insert k v → (a == k) = false → a ∈ m := by
   simpa [mem_iff_contains] using contains_of_contains_insert h
 
 @[simp]
-theorem contains_insert_self [EquivBEq α] [LawfulHashable α] {a : α} {b : β a} : (m.insert a b).contains a := by
+theorem contains_insert_self [EquivBEq α] [LawfulHashable α] {k : α} {v : β k} : (m.insert k v).contains k := by
   dhashmap_simp_to_raw using Raw₀.contains_insert_self
 
 @[simp]
-theorem mem_insert_self [EquivBEq α] [LawfulHashable α] {a : α} {b : β a} : a ∈ m.insert a b := by
+theorem mem_insert_self [EquivBEq α] [LawfulHashable α] {k : α} {v : β k} : k ∈ m.insert k v := by
   simp [mem_iff_contains, contains_insert_self h]
 
 @[simp]
@@ -125,31 +125,31 @@ theorem size_emptyc : (∅ : Raw α β).size = 0 :=
 theorem isEmpty_eq_size_eq_zero : m.isEmpty = (m.size == 0) := by
   simp [isEmpty]
 
-theorem size_insert [EquivBEq α] [LawfulHashable α] {a : α} {b : β a} : (m.insert a b).size = bif m.contains a then m.size else m.size + 1 := by
+theorem size_insert [EquivBEq α] [LawfulHashable α] {k : α} {v : β k} : (m.insert k v).size = bif m.contains k then m.size else m.size + 1 := by
   dhashmap_simp_to_raw using Raw₀.size_insert
 
-theorem size_le_size_insert [EquivBEq α] [LawfulHashable α] {a : α} {b : β a} : m.size ≤ (m.insert a b).size := by
+theorem size_le_size_insert [EquivBEq α] [LawfulHashable α] {k : α} {v : β k} : m.size ≤ (m.insert k v).size := by
   dhashmap_simp_to_raw using Raw₀.size_le_size_insert ⟨m, _⟩ h
 
 @[simp]
-theorem remove_empty {a : α} {c : Nat} : (empty c : Raw α β).remove a = empty c := by
+theorem remove_empty {k : α} {c : Nat} : (empty c : Raw α β).remove k = empty c := by
   rw [remove_eq (by dhashmap_wf_trivial)]
   exact congrArg Subtype.val Raw₀.remove_empty
 
 @[simp]
-theorem remove_emptyc {a : α} : (∅ : Raw α β).remove a = ∅ :=
+theorem remove_emptyc {k : α} : (∅ : Raw α β).remove k = ∅ :=
   remove_empty
 
 @[simp]
-theorem isEmpty_remove [EquivBEq α] [LawfulHashable α] {a : α} : (m.remove a).isEmpty = (m.isEmpty || (m.size == 1 && m.contains a)) := by
+theorem isEmpty_remove [EquivBEq α] [LawfulHashable α] {k : α} : (m.remove k).isEmpty = (m.isEmpty || (m.size == 1 && m.contains k)) := by
   dhashmap_simp_to_raw using Raw₀.isEmpty_remove
 
 @[simp]
-theorem contains_remove [EquivBEq α] [LawfulHashable α] {k a : α} : (m.remove k).contains a = (!(k == a) && m.contains a) := by
+theorem contains_remove [EquivBEq α] [LawfulHashable α] {k a : α} : (m.remove k).contains a = (!(a == k) && m.contains a) := by
   dhashmap_simp_to_raw using Raw₀.contains_remove
 
 @[simp]
-theorem mem_remove [EquivBEq α] [LawfulHashable α] {k a : α} : a ∈ m.remove k ↔ (k == a) = false ∧ a ∈ m := by
+theorem mem_remove [EquivBEq α] [LawfulHashable α] {k a : α} : a ∈ m.remove k ↔ (a == k) = false ∧ a ∈ m := by
   simp [mem_iff_contains, contains_remove h]
 
 theorem contains_of_contains_remove [EquivBEq α] [LawfulHashable α] {k a : α} : (m.remove k).contains a → m.contains a := by
@@ -158,18 +158,18 @@ theorem contains_of_contains_remove [EquivBEq α] [LawfulHashable α] {k a : α}
 theorem mem_of_mem_remove [EquivBEq α] [LawfulHashable α] {k a : α} : a ∈ m.remove k → a ∈ m := by
   simpa [mem_iff_contains] using contains_of_contains_remove h
 
-theorem size_remove [EquivBEq α] [LawfulHashable α] {a : α} : (m.remove a).size = bif m.contains a then m.size - 1 else m.size := by
+theorem size_remove [EquivBEq α] [LawfulHashable α] {k : α} : (m.remove k).size = bif m.contains k then m.size - 1 else m.size := by
   dhashmap_simp_to_raw using Raw₀.size_remove
 
-theorem size_remove_le [EquivBEq α] [LawfulHashable α] {a : α} : (m.remove a).size ≤ m.size := by
+theorem size_remove_le [EquivBEq α] [LawfulHashable α] {k : α} : (m.remove k).size ≤ m.size := by
   dhashmap_simp_to_raw using Raw₀.size_remove_le
 
 @[simp]
-theorem fst_containsThenInsert {a : α} {b : β a} : (m.containsThenInsert a b).1 = m.insert a b := by
+theorem fst_containsThenInsert {k : α} {v : β k} : (m.containsThenInsert k v).1 = m.insert k v := by
   dhashmap_simp_to_raw using congrArg Subtype.val (Raw₀.fst_containsThenInsert _)
 
 @[simp]
-theorem snd_containsThenInsert {a : α} {b : β a} : (m.containsThenInsert a b).2 = m.contains a := by
+theorem snd_containsThenInsert {k : α} {v : β k} : (m.containsThenInsert k v).2 = m.contains k := by
   dhashmap_simp_to_raw using Raw₀.snd_containsThenInsert
 
 @[simp]
@@ -183,12 +183,12 @@ theorem get?_emptyc [LawfulBEq α] {a : α} : (∅ : Raw α β).get? a = none :=
 theorem get?_of_isEmpty [LawfulBEq α] {a : α} : m.isEmpty = true → m.get? a = none := by
   dhashmap_simp_to_raw using Raw₀.get?_of_isEmpty ⟨m, _⟩
 
-theorem get?_insert [LawfulBEq α] {a k : α} {b : β a} :
-    (m.insert a b).get? k = if h : a == k then some (cast (congrArg β (eq_of_beq h)) b) else m.get? k := by
+theorem get?_insert [LawfulBEq α] {a k : α} {v : β k} :
+    (m.insert k v).get? a = if h : a == k then some (cast (congrArg β (eq_of_beq h).symm) v) else m.get? a := by
   dhashmap_simp_to_raw using Raw₀.get?_insert
 
 @[simp]
-theorem get?_insert_self [LawfulBEq α] {a : α} {b : β a} : (m.insert a b).get? a = some b := by
+theorem get?_insert_self [LawfulBEq α] {k : α} {v : β k} : (m.insert k v).get? k = some v := by
   dhashmap_simp_to_raw using Raw₀.get?_insert_self
 
 theorem contains_eq_isSome_get? [LawfulBEq α] {a : α} : m.contains a = (m.get? a).isSome := by
@@ -200,11 +200,11 @@ theorem get?_eq_none_of_contains_eq_false [LawfulBEq α] {a : α} : m.contains a
 theorem get?_eq_none [LawfulBEq α] {a : α} : ¬a ∈ m → m.get? a = none := by
   simpa [mem_iff_contains] using get?_eq_none_of_contains_eq_false h
 
-theorem get?_remove [LawfulBEq α] {a k : α} : (m.remove a).get? k = bif a == k then none else m.get? k := by
+theorem get?_remove [LawfulBEq α] {k a : α} : (m.remove k).get? a = bif a == k then none else m.get? a := by
   dhashmap_simp_to_raw using Raw₀.get?_remove
 
 @[simp]
-theorem get?_remove_self [LawfulBEq α] {a : α} : (m.remove a).get? a = none := by
+theorem get?_remove_self [LawfulBEq α] {k : α} : (m.remove k).get? k = none := by
   dhashmap_simp_to_raw using Raw₀.get?_remove_self
 
 namespace Const
@@ -222,13 +222,13 @@ theorem get?_emptyc {a : α} : get? (∅ : Raw α (fun _ => β)) a = none :=
 theorem get?_of_isEmpty [EquivBEq α] [LawfulHashable α] {a : α} : m.isEmpty = true → get? m a = none := by
   dhashmap_simp_to_raw using Raw₀.Const.get?_of_isEmpty ⟨m, _⟩
 
-theorem get?_insert [EquivBEq α] [LawfulHashable α] {a k : α} {b : β} :
-    get? (m.insert a b) k = bif a == k then some b else get? m k := by
+theorem get?_insert [EquivBEq α] [LawfulHashable α] {k a : α} {v : β} :
+    get? (m.insert k v) a = bif a == k then some v else get? m a := by
   dhashmap_simp_to_raw using Raw₀.Const.get?_insert
 
 @[simp]
-theorem get?_insert_self [EquivBEq α] [LawfulHashable α] {a : α} {b : β} :
-    get? (m.insert a b) a = some b := by
+theorem get?_insert_self [EquivBEq α] [LawfulHashable α] {k : α} {v : β} :
+    get? (m.insert k v) k = some v := by
   dhashmap_simp_to_raw using Raw₀.Const.get?_insert_self
 
 theorem contains_eq_isSome_get? [EquivBEq α] [LawfulHashable α] {a : α} : m.contains a = (get? m a).isSome := by
@@ -241,12 +241,12 @@ theorem get?_eq_none_of_contains_eq_false [EquivBEq α] [LawfulHashable α] {a :
 theorem get?_eq_none [EquivBEq α] [LawfulHashable α] {a : α} : ¬a ∈ m → get? m a = none := by
     simpa [mem_iff_contains] using get?_eq_none_of_contains_eq_false h
 
-theorem get?_remove [EquivBEq α] [LawfulHashable α] {a k : α} :
-    Const.get? (m.remove a) k = bif a == k then none else get? m k := by
+theorem get?_remove [EquivBEq α] [LawfulHashable α] {k a : α} :
+    Const.get? (m.remove k) a = bif a == k then none else get? m a := by
   dhashmap_simp_to_raw using Raw₀.Const.get?_remove
 
 @[simp]
-theorem get?_remove_self [EquivBEq α] [LawfulHashable α] {a : α} : get? (m.remove a) a = none := by
+theorem get?_remove_self [EquivBEq α] [LawfulHashable α] {k : α} : get? (m.remove k) k = none := by
   dhashmap_simp_to_raw using Raw₀.Const.get?_remove_self
 
 theorem get?_eq_get? [LawfulBEq α] {a : α} : get? m a = m.get? a := by
@@ -257,19 +257,19 @@ theorem get?_congr [EquivBEq α] [LawfulHashable α] {a b : α} (hab : a == b) :
 
 end Const
 
-theorem get_insert [LawfulBEq α] {a k : α} {b : β a} {h₁} :
-    (m.insert a b).get k h₁ =
+theorem get_insert [LawfulBEq α] {k a : α} {v : β k} {h₁} :
+    (m.insert k v).get a h₁ =
       if h₂ : a == k then
-        cast (congrArg β (eq_of_beq h₂)) b
+        cast (congrArg β (eq_of_beq h₂).symm) v
       else
-        m.get k (mem_of_mem_insert h h₁ (Bool.eq_false_iff.2 h₂)) := by
+        m.get a (mem_of_mem_insert h h₁ (Bool.eq_false_iff.2 h₂)) := by
   dhashmap_simp_to_raw using Raw₀.get_insert ⟨m, _⟩
 
 @[simp]
-theorem get_insert_self [LawfulBEq α] {a : α} {b : β a} : (m.insert a b).get a (mem_insert_self h) = b := by
+theorem get_insert_self [LawfulBEq α] {k : α} {v : β k} : (m.insert k v).get k (mem_insert_self h) = v := by
   dhashmap_simp_to_raw using Raw₀.get_insert_self ⟨m, _⟩
 
-theorem get_remove [LawfulBEq α] {a k : α} {h'} :
+theorem get_remove [LawfulBEq α] {k a : α} {h'} :
     (m.remove a).get k h' = m.get k (mem_of_mem_remove h h') := by
   dhashmap_simp_to_raw using Raw₀.get_remove ⟨m, _⟩
 
@@ -280,17 +280,17 @@ namespace Const
 
 variable {β : Type v} {m : DHashMap.Raw α (fun _ => β)} (h : m.WF)
 
-theorem get_insert [EquivBEq α] [LawfulHashable α] {a k : α} {b : β} {h₁} :
-    get (m.insert a b) k h₁ = if h₂ : a == k then b else get m k (mem_of_mem_insert h h₁ (Bool.eq_false_iff.2 h₂)) := by
+theorem get_insert [EquivBEq α] [LawfulHashable α] {k a : α} {v : β} {h₁} :
+    get (m.insert k v) a h₁ = if h₂ : a == k then v else get m a (mem_of_mem_insert h h₁ (Bool.eq_false_iff.2 h₂)) := by
   dhashmap_simp_to_raw using Raw₀.Const.get_insert ⟨m, _⟩
 
 @[simp]
-theorem get_insert_self [EquivBEq α] [LawfulHashable α] {a : α} {b : β} :
-    get (m.insert a b) a (mem_insert_self h) = b := by
+theorem get_insert_self [EquivBEq α] [LawfulHashable α] {k : α} {v : β} :
+    get (m.insert k v) k (mem_insert_self h) = v := by
   dhashmap_simp_to_raw using Raw₀.Const.get_insert_self ⟨m, _⟩
 
-theorem get_remove [EquivBEq α] [LawfulHashable α] {a k : α} {h'} :
-    get (m.remove a) k h' = get m k (mem_of_mem_remove h h') := by
+theorem get_remove [EquivBEq α] [LawfulHashable α] {k a : α} {h'} :
+    get (m.remove k) a h' = get m a (mem_of_mem_remove h h') := by
   dhashmap_simp_to_raw using Raw₀.Const.get_remove ⟨m, _⟩
 
 theorem get?_eq_some_get [EquivBEq α] [LawfulHashable α] {a : α} {h : a ∈ m} : get? m a = some (get m a h) := by
@@ -315,13 +315,13 @@ theorem get!_emptyc [LawfulBEq α] {a : α} [Inhabited (β a)] : (∅ : Raw α �
 theorem get!_of_isEmpty [LawfulBEq α] {a : α} [Inhabited (β a)] : m.isEmpty = true → m.get! a = default := by
   dhashmap_simp_to_raw using Raw₀.get!_of_isEmpty ⟨m, _⟩
 
-theorem get!_insert [LawfulBEq α] {a k : α} [Inhabited (β k)] {b : β a} :
-    (m.insert a b).get! k = if h : a == k then cast (congrArg β (eq_of_beq h)) b else m.get! k := by
+theorem get!_insert [LawfulBEq α] {k a : α} [Inhabited (β a)] {v : β k} :
+    (m.insert k v).get! a = if h : a == k then cast (congrArg β (eq_of_beq h).symm) v else m.get! a := by
   dhashmap_simp_to_raw using Raw₀.get!_insert
 
 @[simp]
-theorem get!_insert_self [LawfulBEq α] {a : α} [Inhabited (β a)] {b : β a} :
-    (m.insert a b).get! a = b := by
+theorem get!_insert_self [LawfulBEq α] {k : α} [Inhabited (β k)] {v : β k} :
+    (m.insert k v).get! k = v := by
   dhashmap_simp_to_raw using Raw₀.get!_insert_self
 
 theorem get!_eq_default_of_contains_eq_false [LawfulBEq α] {a : α} [Inhabited (β a)] :
@@ -332,8 +332,8 @@ theorem get!_eq_default [LawfulBEq α] {a : α} [Inhabited (β a)] :
     ¬a ∈ m → m.get! a = default := by
   simpa [mem_iff_contains] using get!_eq_default_of_contains_eq_false h
 
-theorem get!_remove [LawfulBEq α] {a k : α} [Inhabited (β k)] :
-    (m.remove a).get! k = bif a == k then default else m.get! k := by
+theorem get!_remove [LawfulBEq α] {k a : α} [Inhabited (β a)] :
+    (m.remove k).get! a = bif a == k then default else m.get! a := by
   dhashmap_simp_to_raw using Raw₀.get!_remove
 
 @[simp]
@@ -372,13 +372,13 @@ theorem get!_emptyc [Inhabited β] {a : α} : get! (∅ : Raw α (fun _ => β)) 
 theorem get!_of_isEmpty [EquivBEq α] [LawfulHashable α] [Inhabited β] {a : α} : m.isEmpty = true → get! m a = default := by
   dhashmap_simp_to_raw using Raw₀.Const.get!_of_isEmpty ⟨m, _⟩
 
-theorem get!_insert [EquivBEq α] [LawfulHashable α] [Inhabited β] {a k : α} {b : β} :
-    get! (m.insert a b) k = bif a == k then b else get! m k := by
+theorem get!_insert [EquivBEq α] [LawfulHashable α] [Inhabited β] {k a : α} {v : β} :
+    get! (m.insert k v) a = bif a == k then v else get! m a := by
   dhashmap_simp_to_raw using Raw₀.Const.get!_insert
 
 @[simp]
-theorem get!_insert_self [EquivBEq α] [LawfulHashable α] [Inhabited β] {a : α} {b : β} :
-    get! (m.insert a b) a = b := by
+theorem get!_insert_self [EquivBEq α] [LawfulHashable α] [Inhabited β] {k : α} {v : β} :
+    get! (m.insert k v) k = v := by
   dhashmap_simp_to_raw using Raw₀.Const.get!_insert_self
 
 theorem get!_eq_default_of_contains_eq_false [EquivBEq α] [LawfulHashable α] [Inhabited β] {a : α} :
@@ -389,8 +389,8 @@ theorem get!_eq_default [EquivBEq α] [LawfulHashable α] [Inhabited β] {a : α
     ¬a ∈ m → get! m a = default := by
   simpa [mem_iff_contains] using get!_eq_default_of_contains_eq_false h
 
-theorem get!_remove [EquivBEq α] [LawfulHashable α] [Inhabited β] {a k : α} :
-    get! (m.remove a) k = bif a == k then default else get! m k := by
+theorem get!_remove [EquivBEq α] [LawfulHashable α] [Inhabited β] {k a : α} :
+    get! (m.remove k) a = bif a == k then default else get! m a := by
   dhashmap_simp_to_raw using Raw₀.Const.get!_remove
 
 @[simp]
@@ -435,8 +435,8 @@ theorem getD_emptyc [LawfulBEq α] {a : α} {fallback : β a} : (∅ : Raw α β
 theorem getD_of_isEmpty [LawfulBEq α] {a : α} {fallback : β a} : m.isEmpty = true → m.getD a fallback = fallback := by
   dhashmap_simp_to_raw using Raw₀.getD_of_isEmpty ⟨m, _⟩
 
-theorem getD_insert [LawfulBEq α] {a k : α} {fallback : β k} {b : β a} :
-    (m.insert a b).getD k fallback = if h : a == k then cast (congrArg β (eq_of_beq h)) b else m.getD k fallback := by
+theorem getD_insert [LawfulBEq α] {k a : α} {fallback : β a} {v : β k} :
+    (m.insert k v).getD a fallback = if h : a == k then cast (congrArg β (eq_of_beq h).symm) v else m.getD a fallback := by
   dhashmap_simp_to_raw using Raw₀.getD_insert
 
 @[simp]
@@ -452,8 +452,8 @@ theorem getD_eq_fallback [LawfulBEq α] {a : α} {fallback : β a} :
     ¬a ∈ m → m.getD a fallback = fallback := by
   simpa [mem_iff_contains] using getD_eq_fallback_of_contains_eq_false h
 
-theorem getD_remove [LawfulBEq α] {a k : α} {fallback : β k} :
-    (m.remove a).getD k fallback = bif a == k then fallback else m.getD k fallback := by
+theorem getD_remove [LawfulBEq α] {k a : α} {fallback : β a} :
+    (m.remove k).getD a fallback = bif a == k then fallback else m.getD a fallback := by
   dhashmap_simp_to_raw using Raw₀.getD_remove
 
 @[simp]
@@ -496,13 +496,13 @@ theorem getD_emptyc {a : α} {fallback : β} : getD (∅ : Raw α (fun _ => β))
 theorem getD_of_isEmpty [EquivBEq α] [LawfulHashable α] {a : α} {fallback : β} : m.isEmpty = true → getD m a fallback = fallback := by
   dhashmap_simp_to_raw using Raw₀.Const.getD_of_isEmpty ⟨m, _⟩
 
-theorem getD_insert [EquivBEq α] [LawfulHashable α] {a k : α} {fallback b : β} :
-    getD (m.insert a b) k fallback = bif a == k then b else getD m k fallback := by
+theorem getD_insert [EquivBEq α] [LawfulHashable α] {k a : α} {fallback v : β} :
+    getD (m.insert k v) a fallback = bif a == k then v else getD m a fallback := by
   dhashmap_simp_to_raw using Raw₀.Const.getD_insert
 
 @[simp]
-theorem getD_insert_self [EquivBEq α] [LawfulHashable α] {a : α} {fallback b : β} :
-   getD (m.insert a b) a fallback = b := by
+theorem getD_insert_self [EquivBEq α] [LawfulHashable α] {k : α} {fallback v : β} :
+   getD (m.insert k v) k fallback = v := by
   dhashmap_simp_to_raw using Raw₀.Const.getD_insert_self
 
 theorem getD_eq_fallback_of_contains_eq_false [EquivBEq α] [LawfulHashable α] {a : α} {fallback : β} :
@@ -513,8 +513,8 @@ theorem getD_eq_fallback [EquivBEq α] [LawfulHashable α] {a : α} {fallback : 
     ¬a ∈ m → getD m a fallback = fallback := by
   simpa [mem_iff_contains] using getD_eq_fallback_of_contains_eq_false h
 
-theorem getD_remove [EquivBEq α] [LawfulHashable α] {a k : α} {fallback : β} :
-    getD (m.remove a) k fallback = bif a == k then fallback else getD m k fallback := by
+theorem getD_remove [EquivBEq α] [LawfulHashable α] {k a : α} {fallback : β} :
+    getD (m.remove k) a fallback = bif a == k then fallback else getD m a fallback := by
   dhashmap_simp_to_raw using Raw₀.Const.getD_remove
 
 @[simp]
@@ -553,58 +553,58 @@ theorem getD_congr [EquivBEq α] [LawfulHashable α] {a b : α} {fallback : β} 
 end Const
 
 @[simp]
-theorem isEmpty_insertIfNew [EquivBEq α] [LawfulHashable α] {a : α} {b : β a} :
-    (m.insertIfNew a b).isEmpty = false := by
+theorem isEmpty_insertIfNew [EquivBEq α] [LawfulHashable α] {k : α} {v : β k} :
+    (m.insertIfNew k v).isEmpty = false := by
   dhashmap_simp_to_raw using Raw₀.isEmpty_insertIfNew
 
 @[simp]
-theorem contains_insertIfNew [EquivBEq α] [LawfulHashable α] {a k : α} {b : β a} :
-    (m.insertIfNew a b).contains k = (a == k || m.contains k) := by
+theorem contains_insertIfNew [EquivBEq α] [LawfulHashable α] {k a : α} {v : β k} :
+    (m.insertIfNew k v).contains a = (a == k || m.contains a) := by
   dhashmap_simp_to_raw using Raw₀.contains_insertIfNew
 
 @[simp]
-theorem mem_insertIfNew [EquivBEq α] [LawfulHashable α] {a k : α} {b : β a} :
-    k ∈ m.insertIfNew a b ↔ a == k ∨ k ∈ m := by
+theorem mem_insertIfNew [EquivBEq α] [LawfulHashable α] {k a : α} {v : β k} :
+    a ∈ m.insertIfNew k v ↔ a == k ∨ a ∈ m := by
   simp [mem_iff_contains, contains_insertIfNew h]
 
 /-- This is a restatement of `contains_insertIfNew` that is written to exactly match the proof obligation in the statement of
     `get_insertIfNew`. -/
-theorem contains_of_contains_insertIfNew [EquivBEq α] [LawfulHashable α] {a k : α} {b : β a} :
-    (m.insertIfNew a b).contains k → ¬((a == k) ∧ m.contains a = false) → m.contains k := by
+theorem contains_of_contains_insertIfNew [EquivBEq α] [LawfulHashable α] {k a : α} {v : β k} :
+    (m.insertIfNew k v).contains a → ¬((a == k) ∧ m.contains k = false) → m.contains a := by
   dhashmap_simp_to_raw using Raw₀.contains_of_contains_insertIfNew
 
 /-- This is a restatement of `mem_insertIfNew` that is written to exactly match the proof obligation in the statement of
     `get_insertIfNew`. -/
-theorem mem_of_mem_insertIfNew [EquivBEq α] [LawfulHashable α] {a k : α} {b : β a} :
-    k ∈ m.insertIfNew a b → ¬((a == k) ∧ ¬a ∈ m) → k ∈ m := by
+theorem mem_of_mem_insertIfNew [EquivBEq α] [LawfulHashable α] {k a : α} {v : β k} :
+    a ∈ m.insertIfNew k v → ¬((a == k) ∧ ¬k ∈ m) → a ∈ m := by
   simpa [mem_iff_contains] using contains_of_contains_insertIfNew h
 
-theorem size_insertIfNew [EquivBEq α] [LawfulHashable α] {a : α} {b : β a} :
-    (m.insertIfNew a b).size = bif m.contains a then m.size else m.size + 1 := by
+theorem size_insertIfNew [EquivBEq α] [LawfulHashable α] {k : α} {v : β k} :
+    (m.insertIfNew k v).size = bif m.contains k then m.size else m.size + 1 := by
   dhashmap_simp_to_raw using Raw₀.size_insertIfNew
 
-theorem size_le_size_insertIfNew [EquivBEq α] [LawfulHashable α] {a : α} {b : β a} :
-    m.size ≤ (m.insertIfNew a b).size := by
+theorem size_le_size_insertIfNew [EquivBEq α] [LawfulHashable α] {k : α} {v : β k} :
+    m.size ≤ (m.insertIfNew k v).size := by
   dhashmap_simp_to_raw using Raw₀.size_le_size_insertIfNew ⟨m, _⟩
 
-theorem get?_insertIfNew [LawfulBEq α] {a k : α} {b : β a} :
-    (m.insertIfNew a b).get? k = if h : a == k ∧ ¬a ∈ m then some (cast (congrArg β (eq_of_beq h.1)) b) else m.get? k := by
+theorem get?_insertIfNew [LawfulBEq α] {k a : α} {v : β k} :
+    (m.insertIfNew k v).get? a = if h : a == k ∧ ¬k ∈ m then some (cast (congrArg β (eq_of_beq h.1).symm) v) else m.get? a := by
   simp only [mem_iff_contains, Bool.not_eq_true]
   dhashmap_simp_to_raw using Raw₀.get?_insertIfNew ⟨m, _⟩
 
-theorem get_insertIfNew [LawfulBEq α] {a k : α} {b : β a} {h₁} :
-    (m.insertIfNew a b).get k h₁ = if h₂ : a == k ∧ ¬a ∈ m then cast (congrArg β (eq_of_beq h₂.1)) b else m.get k
+theorem get_insertIfNew [LawfulBEq α] {k a : α} {v : β k} {h₁} :
+    (m.insertIfNew k v).get a h₁ = if h₂ : a == k ∧ ¬k ∈ m then cast (congrArg β (eq_of_beq h₂.1).symm) v else m.get a
       (mem_of_mem_insertIfNew h h₁ h₂) := by
   simp only [mem_iff_contains, Bool.not_eq_true]
   dhashmap_simp_to_raw using Raw₀.get_insertIfNew ⟨m, _⟩
 
-theorem get!_insertIfNew [LawfulBEq α] {a k : α} [Inhabited (β k)] {b : β a} :
-    (m.insertIfNew a b).get! k = if h : a == k ∧ ¬a ∈ m then cast (congrArg β (eq_of_beq h.1)) b else m.get! k := by
+theorem get!_insertIfNew [LawfulBEq α] {k a : α} [Inhabited (β a)] {v : β k} :
+    (m.insertIfNew k v).get! a = if h : a == k ∧ ¬k ∈ m then cast (congrArg β (eq_of_beq h.1).symm) v else m.get! a := by
   simp only [mem_iff_contains, Bool.not_eq_true]
   dhashmap_simp_to_raw using Raw₀.get!_insertIfNew ⟨m, _⟩
 
-theorem getD_insertIfNew [LawfulBEq α] {a k : α} {fallback : β k} {b : β a} :
-    (m.insertIfNew a b).getD k fallback = if h : a == k ∧ ¬a ∈ m then cast (congrArg β (eq_of_beq h.1)) b else m.getD k fallback := by
+theorem getD_insertIfNew [LawfulBEq α] {k a : α} {fallback : β a} {v : β k} :
+    (m.insertIfNew k v).getD a fallback = if h : a == k ∧ ¬k ∈ m then cast (congrArg β (eq_of_beq h.1).symm) v else m.getD a fallback := by
   simp only [mem_iff_contains, Bool.not_eq_true]
   dhashmap_simp_to_raw using Raw₀.getD_insertIfNew
 
@@ -612,31 +612,31 @@ namespace Const
 
 variable {β : Type v} {m : DHashMap.Raw α (fun _ => β)} (h : m.WF)
 
-theorem get?_insertIfNew [EquivBEq α] [LawfulHashable α] {a k : α} {b : β} :
-    get? (m.insertIfNew a b) k = bif a == k && !m.contains a then some b else get? m k := by
+theorem get?_insertIfNew [EquivBEq α] [LawfulHashable α] {k a : α} {v : β} :
+    get? (m.insertIfNew k v) a = bif a == k && !m.contains k then some v else get? m a := by
   dhashmap_simp_to_raw using Raw₀.Const.get?_insertIfNew
 
-theorem get_insertIfNew [EquivBEq α] [LawfulHashable α] {a k : α} {b : β} {h₁} :
-    get (m.insertIfNew a b) k h₁ = if h₂ : a == k ∧ ¬a ∈ m then b else get m k (mem_of_mem_insertIfNew h h₁ h₂) := by
+theorem get_insertIfNew [EquivBEq α] [LawfulHashable α] {k a : α} {v : β} {h₁} :
+    get (m.insertIfNew k v) a h₁ = if h₂ : a == k ∧ ¬k ∈ m then v else get m a (mem_of_mem_insertIfNew h h₁ h₂) := by
   simp only [mem_iff_contains, Bool.not_eq_true]
   dhashmap_simp_to_raw using Raw₀.Const.get_insertIfNew ⟨m, _⟩
 
-theorem get!_insertIfNew [EquivBEq α] [LawfulHashable α] [Inhabited β] {a k : α} {b : β} :
-    get! (m.insertIfNew a b) k = bif a == k && !m.contains a then b else get! m k := by
+theorem get!_insertIfNew [EquivBEq α] [LawfulHashable α] [Inhabited β] {k a : α} {v : β} :
+    get! (m.insertIfNew k v) a = bif a == k && !m.contains k then v else get! m a := by
   dhashmap_simp_to_raw using Raw₀.Const.get!_insertIfNew
 
-theorem getD_insertIfNew [EquivBEq α] [LawfulHashable α] {a k : α} {fallback b : β} :
-    getD (m.insertIfNew a b) k fallback = bif a == k && !m.contains a then b else getD m k fallback := by
+theorem getD_insertIfNew [EquivBEq α] [LawfulHashable α] {k a : α} {fallback v : β} :
+    getD (m.insertIfNew k v) a fallback = bif a == k && !m.contains k then v else getD m a fallback := by
   dhashmap_simp_to_raw using Raw₀.Const.getD_insertIfNew
 
 end Const
 
 @[simp]
-theorem fst_getThenInsertIfNew? [LawfulBEq α] {a : α} {b : β a} : (m.getThenInsertIfNew? a b).1 = m.insertIfNew a b := by
+theorem fst_getThenInsertIfNew? [LawfulBEq α] {k : α} {v : β k} : (m.getThenInsertIfNew? k v).1 = m.insertIfNew k v := by
   dhashmap_simp_to_raw using congrArg Subtype.val (Raw₀.fst_getThenInsertIfNew? _)
 
 @[simp]
-theorem snd_getThenInsertIfNew? [LawfulBEq α] {a : α} {b : β a} : (m.getThenInsertIfNew? a b).2 = m.get? a := by
+theorem snd_getThenInsertIfNew? [LawfulBEq α] {k : α} {v : β k} : (m.getThenInsertIfNew? k v).2 = m.get? k := by
   dhashmap_simp_to_raw using Raw₀.snd_getThenInsertIfNew?
 
 namespace Const
@@ -644,11 +644,11 @@ namespace Const
 variable {β : Type v} {m : DHashMap.Raw α (fun _ => β)} (h : m.WF)
 
 @[simp]
-theorem fst_getThenInsertIfNew? {a : α} {b : β} : (getThenInsertIfNew? m a b).1 = m.insertIfNew a b := by
+theorem fst_getThenInsertIfNew? {k : α} {v : β} : (getThenInsertIfNew? m k v).1 = m.insertIfNew k v := by
   dhashmap_simp_to_raw using congrArg Subtype.val (Raw₀.Const.fst_getThenInsertIfNew? _)
 
 @[simp]
-theorem snd_getThenInsertIfNew? {a : α} {b : β} : (getThenInsertIfNew? m a b).2 = get? m a := by
+theorem snd_getThenInsertIfNew? {k : α} {v : β} : (getThenInsertIfNew? m k v).2 = get? m k := by
   dhashmap_simp_to_raw using Raw₀.Const.snd_getThenInsertIfNew?
 
 end Const
@@ -668,7 +668,7 @@ theorem isEmpty_emptyc : (∅ : DHashMap α β).isEmpty :=
   isEmpty_empty
 
 @[simp]
-theorem isEmpty_insert [EquivBEq α] [LawfulHashable α] {a : α} {b : β a} : (m.insert a b).isEmpty = false :=
+theorem isEmpty_insert [EquivBEq α] [LawfulHashable α] {k : α} {v : β k} : (m.insert k v).isEmpty = false :=
   Raw₀.isEmpty_insert _ m.2
 
 theorem contains_congr [EquivBEq α] [LawfulHashable α] {a b : α} (hab : a == b) : m.contains a = m.contains b :=
@@ -693,27 +693,27 @@ theorem mem_congr [EquivBEq α] [LawfulHashable α] {a b : α} (hab : a == b) : 
   not_mem_empty
 
 @[simp]
-theorem contains_insert [EquivBEq α] [LawfulHashable α] {a k : α} {b : β a} : (m.insert a b).contains k = (a == k || m.contains k) :=
+theorem contains_insert [EquivBEq α] [LawfulHashable α] {k a : α} {v : β k} : (m.insert k v).contains a = (a == k || m.contains a) :=
   Raw₀.contains_insert ⟨m.1, _⟩ m.2
 
 @[simp]
-theorem mem_insert [EquivBEq α] [LawfulHashable α] {a k : α} {b : β a} : k ∈ m.insert a b ↔ a == k ∨ k ∈ m := by
+theorem mem_insert [EquivBEq α] [LawfulHashable α] {k a : α} {v : β k} : a ∈ m.insert k v ↔ a == k ∨ a ∈ m := by
   simp [mem_iff_contains, contains_insert]
 
-theorem contains_of_contains_insert [EquivBEq α] [LawfulHashable α] {a k : α} {b : β a} :
-    (m.insert a b).contains k → (a == k) = false → m.contains k :=
+theorem contains_of_contains_insert [EquivBEq α] [LawfulHashable α] {k a : α} {v : β k} :
+    (m.insert k v).contains a → (a == k) = false → m.contains a :=
   Raw₀.contains_of_contains_insert ⟨m.1, _⟩ m.2
 
-theorem mem_of_mem_insert [EquivBEq α] [LawfulHashable α] {a k : α} {b : β a} :
-    k ∈ m.insert a b → (a == k) = false → k ∈ m := by
+theorem mem_of_mem_insert [EquivBEq α] [LawfulHashable α] {k a : α} {v : β k} :
+    a ∈ m.insert k v → (a == k) = false → a ∈ m := by
   simpa [mem_iff_contains, -contains_insert] using contains_of_contains_insert
 
 @[simp]
-theorem contains_insert_self [EquivBEq α] [LawfulHashable α] {a : α} {b : β a} : (m.insert a b).contains a :=
+theorem contains_insert_self [EquivBEq α] [LawfulHashable α] {k : α} {v : β k} : (m.insert k v).contains k :=
   Raw₀.contains_insert_self ⟨m.1, _⟩ m.2
 
 @[simp]
-theorem mem_insert_self [EquivBEq α] [LawfulHashable α] {a : α} {b : β a} : a ∈ m.insert a b := by
+theorem mem_insert_self [EquivBEq α] [LawfulHashable α] {k : α} {v : β k} : k ∈ m.insert k v := by
   simp [mem_iff_contains, contains_insert_self]
 
 @[simp]
@@ -726,32 +726,32 @@ theorem size_emptyc : (∅ : DHashMap α β).size = 0 :=
 
 theorem isEmpty_eq_size_eq_zero : m.isEmpty = (m.size == 0) := rfl
 
-theorem size_insert [EquivBEq α] [LawfulHashable α] {a : α} {b : β a} :
-    (m.insert a b).size = bif m.contains a then m.size else m.size + 1 :=
+theorem size_insert [EquivBEq α] [LawfulHashable α] {k : α} {v : β k} :
+    (m.insert k v).size = bif m.contains k then m.size else m.size + 1 :=
   Raw₀.size_insert ⟨m.1, _⟩ m.2
 
-theorem size_le_size_insert [EquivBEq α] [LawfulHashable α] {a : α} {b : β a} : m.size ≤ (m.insert a b).size :=
+theorem size_le_size_insert [EquivBEq α] [LawfulHashable α] {k : α} {v : β k} : m.size ≤ (m.insert k v).size :=
   Raw₀.size_le_size_insert ⟨m.1, _⟩ m.2
 
 @[simp]
-theorem remove_empty {a : α} {c : Nat} : (empty c : DHashMap α β).remove a = empty c :=
-  Subtype.eq <| (congrArg Subtype.val Raw₀.remove_empty).trans rfl -- TODO WTF?
+theorem remove_empty {k : α} {c : Nat} : (empty c : DHashMap α β).remove k = empty c :=
+  Subtype.eq (congrArg Subtype.val (Raw₀.remove_empty (k := k)) :) -- Lean code is happy
 
 @[simp]
-theorem remove_emptyc {a : α} : (∅ : DHashMap α β).remove a = ∅ :=
+theorem remove_emptyc {k : α} : (∅ : DHashMap α β).remove k = ∅ :=
   remove_empty
 
 @[simp]
-theorem isEmpty_remove [EquivBEq α] [LawfulHashable α] {a : α} :
-    (m.remove a).isEmpty = (m.isEmpty || (m.size == 1 && m.contains a)) :=
+theorem isEmpty_remove [EquivBEq α] [LawfulHashable α] {k : α} :
+    (m.remove k).isEmpty = (m.isEmpty || (m.size == 1 && m.contains k)) :=
   Raw₀.isEmpty_remove _ m.2
 
 @[simp]
-theorem contains_remove [EquivBEq α] [LawfulHashable α] {k a : α} : (m.remove k).contains a = (!(k == a) && m.contains a) :=
+theorem contains_remove [EquivBEq α] [LawfulHashable α] {k a : α} : (m.remove k).contains a = (!(a == k) && m.contains a) :=
   Raw₀.contains_remove ⟨m.1, _⟩ m.2
 
 @[simp]
-theorem mem_remove [EquivBEq α] [LawfulHashable α] {k a : α} : a ∈ m.remove k ↔ (k == a) = false ∧ a ∈ m := by
+theorem mem_remove [EquivBEq α] [LawfulHashable α] {k a : α} : a ∈ m.remove k ↔ (a == k) = false ∧ a ∈ m := by
   simp [mem_iff_contains, contains_remove]
 
 theorem contains_of_contains_remove [EquivBEq α] [LawfulHashable α] {k a : α} : (m.remove k).contains a → m.contains a :=
@@ -760,18 +760,18 @@ theorem contains_of_contains_remove [EquivBEq α] [LawfulHashable α] {k a : α}
 theorem mem_of_mem_remove [EquivBEq α] [LawfulHashable α] {k a : α} : a ∈ m.remove k → a ∈ m := by
   simp
 
-theorem size_remove [EquivBEq α] [LawfulHashable α] {a : α} : (m.remove a).size = bif m.contains a then m.size - 1 else m.size :=
+theorem size_remove [EquivBEq α] [LawfulHashable α] {k : α} : (m.remove k).size = bif m.contains k then m.size - 1 else m.size :=
   Raw₀.size_remove _ m.2
 
-theorem size_remove_le [EquivBEq α] [LawfulHashable α] {a : α} : (m.remove a).size ≤ m.size :=
+theorem size_remove_le [EquivBEq α] [LawfulHashable α] {k : α} : (m.remove k).size ≤ m.size :=
   Raw₀.size_remove_le _ m.2
 
 @[simp]
-theorem fst_containsThenInsert {a : α} {b : β a} : (m.containsThenInsert a b).1 = m.insert a b :=
+theorem fst_containsThenInsert {k : α} {v : β k} : (m.containsThenInsert k v).1 = m.insert k v :=
   Subtype.eq <| (congrArg Subtype.val (Raw₀.fst_containsThenInsert _)).trans rfl
 
 @[simp]
-theorem snd_containsThenInsert {a : α} {b : β a} : (m.containsThenInsert a b).2 = m.contains a :=
+theorem snd_containsThenInsert {k : α} {v : β k} : (m.containsThenInsert k v).2 = m.contains k :=
   Raw₀.snd_containsThenInsert _
 
 @[simp]
@@ -785,12 +785,12 @@ theorem get?_emptyc [LawfulBEq α] {a : α} : (∅ : DHashMap α β).get? a = no
 theorem get?_of_isEmpty [LawfulBEq α] {a : α} : m.isEmpty = true → m.get? a = none :=
   Raw₀.get?_of_isEmpty ⟨m.1, _⟩ m.2
 
-theorem get?_insert [LawfulBEq α] {a k : α} {b : β a} :
-    (m.insert a b).get? k = if h : a == k then some (cast (congrArg β (eq_of_beq h)) b) else m.get? k :=
+theorem get?_insert [LawfulBEq α] {a k : α} {v : β k} :
+    (m.insert k v).get? a = if h : a == k then some (cast (congrArg β (eq_of_beq h).symm) v) else m.get? a :=
   Raw₀.get?_insert ⟨m.1, _⟩ m.2
 
 @[simp]
-theorem get?_insert_self [LawfulBEq α] {a : α} {b : β a} : (m.insert a b).get? a = some b :=
+theorem get?_insert_self [LawfulBEq α] {k : α} {v : β k} : (m.insert k v).get? k = some v :=
   Raw₀.get?_insert_self ⟨m.1, _⟩ m.2
 
 theorem contains_eq_isSome_get? [LawfulBEq α] {a : α} : m.contains a = (m.get? a).isSome :=
@@ -802,11 +802,11 @@ theorem get?_eq_none_of_contains_eq_false [LawfulBEq α] {a : α} : m.contains a
 theorem get?_eq_none [LawfulBEq α] {a : α} : ¬a ∈ m → m.get? a = none := by
   simpa [mem_iff_contains] using get?_eq_none_of_contains_eq_false
 
-theorem get?_remove [LawfulBEq α] {a k : α} : (m.remove a).get? k = bif a == k then none else m.get? k :=
+theorem get?_remove [LawfulBEq α] {k a : α} : (m.remove k).get? a = bif a == k then none else m.get? a :=
   Raw₀.get?_remove ⟨m.1, _⟩ m.2
 
 @[simp]
-theorem get?_remove_self [LawfulBEq α] {a : α} : (m.remove a).get? a = none :=
+theorem get?_remove_self [LawfulBEq α] {k : α} : (m.remove k).get? k = none :=
   Raw₀.get?_remove_self ⟨m.1, _⟩ m.2
 
 namespace Const
@@ -824,13 +824,13 @@ theorem get?_emptyc {a : α} : get? (∅ : DHashMap α (fun _ => β)) a = none :
 theorem get?_of_isEmpty [EquivBEq α] [LawfulHashable α] {a : α} : m.isEmpty = true → get? m a = none :=
   Raw₀.Const.get?_of_isEmpty ⟨m.1, _⟩ m.2
 
-theorem get?_insert [EquivBEq α] [LawfulHashable α] {a k : α} {b : β} :
-    get? (m.insert a b) k = bif a == k then some b else get? m k :=
+theorem get?_insert [EquivBEq α] [LawfulHashable α] {k a : α} {v : β} :
+    get? (m.insert k v) a = bif a == k then some v else get? m a :=
   Raw₀.Const.get?_insert ⟨m.1, _⟩ m.2
 
 @[simp]
-theorem get?_insert_self [EquivBEq α] [LawfulHashable α] {a : α} {b : β} :
-    get? (m.insert a b) a = some b :=
+theorem get?_insert_self [EquivBEq α] [LawfulHashable α] {k : α} {v : β} :
+    get? (m.insert k v) k = some v :=
   Raw₀.Const.get?_insert_self ⟨m.1, _⟩ m.2
 
 theorem contains_eq_isSome_get? [EquivBEq α] [LawfulHashable α] {a : α} : m.contains a = (get? m a).isSome :=
@@ -842,12 +842,12 @@ theorem get?_eq_none_of_contains_eq_false [EquivBEq α] [LawfulHashable α] {a :
 theorem get?_eq_none [EquivBEq α] [LawfulHashable α] {a : α } : ¬a ∈ m → get? m a = none := by
   simpa [mem_iff_contains] using get?_eq_none_of_contains_eq_false
 
-theorem get?_remove [EquivBEq α] [LawfulHashable α] {a k : α} :
-    Const.get? (m.remove a) k = bif a == k then none else get? m k :=
+theorem get?_remove [EquivBEq α] [LawfulHashable α] {k a : α} :
+    Const.get? (m.remove k) a = bif a == k then none else get? m a :=
   Raw₀.Const.get?_remove ⟨m.1, _⟩ m.2
 
 @[simp]
-theorem get?_remove_self [EquivBEq α] [LawfulHashable α] {a : α} : get? (m.remove a) a = none :=
+theorem get?_remove_self [EquivBEq α] [LawfulHashable α] {k : α} : get? (m.remove k) k = none :=
   Raw₀.Const.get?_remove_self ⟨m.1, _⟩ m.2
 
 theorem get?_eq_get? [LawfulBEq α] {a : α} : get? m a = m.get? a :=
@@ -858,20 +858,20 @@ theorem get?_congr [EquivBEq α] [LawfulHashable α] {a b : α} (hab : a == b) :
 
 end Const
 
-theorem get_insert [LawfulBEq α] {a k : α} {b : β a} {h₁} :
-    (m.insert a b).get k h₁ =
+theorem get_insert [LawfulBEq α] {k a : α} {v : β k} {h₁} :
+    (m.insert k v).get a h₁ =
       if h₂ : a == k then
-        cast (congrArg β (eq_of_beq h₂)) b
+        cast (congrArg β (eq_of_beq h₂).symm) v
       else
-        m.get k (mem_of_mem_insert h₁ (Bool.eq_false_iff.2 h₂)) :=
+        m.get a (mem_of_mem_insert h₁ (Bool.eq_false_iff.2 h₂)) :=
   Raw₀.get_insert ⟨m.1, _⟩ m.2
 
 @[simp]
-theorem get_insert_self [LawfulBEq α] {a : α} {b : β a} : (m.insert a b).get a mem_insert_self = b :=
+theorem get_insert_self [LawfulBEq α] {k : α} {v : β k} : (m.insert k v).get k mem_insert_self = v :=
   Raw₀.get_insert_self ⟨m.1, _⟩ m.2
 
-theorem get_remove [LawfulBEq α] {a k : α} {h'} :
-    (m.remove a).get k h' = m.get k (mem_of_mem_remove h') :=
+theorem get_remove [LawfulBEq α] {k a : α} {h'} :
+    (m.remove k).get a h' = m.get a (mem_of_mem_remove h') :=
   Raw₀.get_remove ⟨m.1, _⟩ m.2
 
 theorem get?_eq_some_get [LawfulBEq α] {a : α} {h} : m.get? a = some (m.get a h) :=
@@ -881,17 +881,17 @@ namespace Const
 
 variable {β : Type v} {m : DHashMap α (fun _ => β)}
 
-theorem get_insert [EquivBEq α] [LawfulHashable α] {a k : α} {b : β} {h₁} :
-    get (m.insert a b) k h₁ = if h₂ : a == k then b else get m k (mem_of_mem_insert h₁ (Bool.eq_false_iff.2 h₂)) :=
+theorem get_insert [EquivBEq α] [LawfulHashable α] {k a : α} {v : β} {h₁} :
+    get (m.insert k v) a h₁ = if h₂ : a == k then v else get m a (mem_of_mem_insert h₁ (Bool.eq_false_iff.2 h₂)) :=
   Raw₀.Const.get_insert ⟨m.1, _⟩ m.2
 
 @[simp]
-theorem get_insert_self [EquivBEq α] [LawfulHashable α] {a : α} {b : β} :
-    get (m.insert a b) a mem_insert_self = b :=
+theorem get_insert_self [EquivBEq α] [LawfulHashable α] {k : α} {v : β} :
+    get (m.insert k v) k mem_insert_self = v :=
   Raw₀.Const.get_insert_self ⟨m.1, _⟩ m.2
 
-theorem get_remove [EquivBEq α] [LawfulHashable α] {a k : α} {h'} :
-    get (m.remove a) k h' = get m k (mem_of_mem_remove h') :=
+theorem get_remove [EquivBEq α] [LawfulHashable α] {k a : α} {h'} :
+    get (m.remove k) a h' = get m a (mem_of_mem_remove h') :=
   Raw₀.Const.get_remove ⟨m.1, _⟩ m.2
 
 theorem get?_eq_some_get [EquivBEq α] [LawfulHashable α] {a : α} {h} : get? m a = some (get m a h) :=
@@ -916,8 +916,8 @@ theorem get!_emptyc [LawfulBEq α] {a : α} [Inhabited (β a)] : (∅ : DHashMap
 theorem get!_of_isEmpty [LawfulBEq α] {a : α} [Inhabited (β a)] : m.isEmpty = true → m.get! a = default :=
   Raw₀.get!_of_isEmpty ⟨m.1, _⟩ m.2
 
-theorem get!_insert [LawfulBEq α] {a k : α} [Inhabited (β k)] {b : β a} :
-    (m.insert a b).get! k = if h : a == k then cast (congrArg β (eq_of_beq h)) b else m.get! k :=
+theorem get!_insert [LawfulBEq α] {k a : α} [Inhabited (β a)] {v : β k} :
+    (m.insert k v).get! a = if h : a == k then cast (congrArg β (eq_of_beq h).symm) v else m.get! a :=
   Raw₀.get!_insert ⟨m.1, _⟩ m.2
 
 @[simp]
@@ -933,8 +933,8 @@ theorem get!_eq_default [LawfulBEq α] {a : α} [Inhabited (β a)] :
     ¬a ∈ m → m.get! a = default := by
   simpa [mem_iff_contains] using get!_eq_default_of_contains_eq_false
 
-theorem get!_remove [LawfulBEq α] {a k : α} [Inhabited (β k)] :
-    (m.remove a).get! k = bif a == k then default else m.get! k :=
+theorem get!_remove [LawfulBEq α] {k a : α} [Inhabited (β a)] :
+    (m.remove k).get! a = bif a == k then default else m.get! a :=
   Raw₀.get!_remove ⟨m.1, _⟩ m.2
 
 @[simp]
@@ -973,13 +973,13 @@ theorem get!_emptyc [Inhabited β] {a : α} : get! (∅ : DHashMap α (fun _ => 
 theorem get!_of_isEmpty [EquivBEq α] [LawfulHashable α] [Inhabited β] {a : α} : m.isEmpty = true → get! m a = default :=
   Raw₀.Const.get!_of_isEmpty ⟨m.1, _⟩ m.2
 
-theorem get!_insert [EquivBEq α] [LawfulHashable α] [Inhabited β] {a k : α} {b : β} :
-    get! (m.insert a b) k = bif a == k then b else get! m k :=
+theorem get!_insert [EquivBEq α] [LawfulHashable α] [Inhabited β] {k a : α} {v : β} :
+    get! (m.insert k v) a = bif a == k then v else get! m a :=
   Raw₀.Const.get!_insert ⟨m.1, _⟩ m.2
 
 @[simp]
-theorem get!_insert_self [EquivBEq α] [LawfulHashable α] [Inhabited β] {a : α} {b : β} :
-    get! (m.insert a b) a = b :=
+theorem get!_insert_self [EquivBEq α] [LawfulHashable α] [Inhabited β] {k : α} {v : β} :
+    get! (m.insert k v) k = v :=
   Raw₀.Const.get!_insert_self ⟨m.1, _⟩ m.2
 
 theorem get!_eq_default_of_contains_eq_false [EquivBEq α] [LawfulHashable α] [Inhabited β] {a : α} :
@@ -990,8 +990,8 @@ theorem get!_eq_default [EquivBEq α] [LawfulHashable α] [Inhabited β] {a : α
     ¬a ∈ m → get! m a = default := by
   simpa [mem_iff_contains] using get!_eq_default_of_contains_eq_false
 
-theorem get!_remove [EquivBEq α] [LawfulHashable α] [Inhabited β] {a k : α} :
-    get! (m.remove a) k = bif a == k then default else get! m k :=
+theorem get!_remove [EquivBEq α] [LawfulHashable α] [Inhabited β] {k a : α} :
+    get! (m.remove k) a = bif a == k then default else get! m a :=
   Raw₀.Const.get!_remove ⟨m.1, _⟩ m.2
 
 @[simp]
@@ -1036,13 +1036,13 @@ theorem getD_emptyc [LawfulBEq α] {a : α} {fallback : β a} : (∅ : DHashMap 
 theorem getD_of_isEmpty [LawfulBEq α] {a : α} {fallback : β a} : m.isEmpty = true → m.getD a fallback = fallback :=
   Raw₀.getD_of_isEmpty ⟨m.1, _⟩ m.2
 
-theorem getD_insert [LawfulBEq α] {a k : α} {fallback : β k} {b : β a} :
-    (m.insert a b).getD k fallback = if h : a == k then cast (congrArg β (eq_of_beq h)) b else m.getD k fallback :=
+theorem getD_insert [LawfulBEq α] {k a : α} {fallback : β a} {v : β k} :
+    (m.insert k v).getD a fallback = if h : a == k then cast (congrArg β (eq_of_beq h).symm) v else m.getD a fallback :=
   Raw₀.getD_insert ⟨m.1, _⟩ m.2
 
 @[simp]
-theorem getD_insert_self [LawfulBEq α] {a : α} {fallback b : β a} :
-    (m.insert a b).getD a fallback = b :=
+theorem getD_insert_self [LawfulBEq α] {k : α} {fallback v : β k} :
+    (m.insert k v).getD k fallback = v :=
   Raw₀.getD_insert_self ⟨m.1, _⟩ m.2
 
 theorem getD_eq_fallback_of_contains_eq_false [LawfulBEq α] {a : α} {fallback : β a} :
@@ -1053,8 +1053,8 @@ theorem getD_eq_fallback [LawfulBEq α] {a : α} {fallback : β a} :
     ¬a ∈ m → m.getD a fallback = fallback := by
   simpa [mem_iff_contains] using getD_eq_fallback_of_contains_eq_false
 
-theorem getD_remove [LawfulBEq α] {a k : α} {fallback : β k} :
-    (m.remove a).getD k fallback = bif a == k then fallback else m.getD k fallback :=
+theorem getD_remove [LawfulBEq α] {k a : α} {fallback : β a} :
+    (m.remove k).getD a fallback = bif a == k then fallback else m.getD a fallback :=
   Raw₀.getD_remove ⟨m.1, _⟩ m.2
 
 @[simp]
@@ -1097,13 +1097,13 @@ theorem getD_emptyc {a : α} {fallback : β} : getD (∅ : DHashMap α (fun _ =>
 theorem getD_of_isEmpty [EquivBEq α] [LawfulHashable α] {a : α} {fallback : β} : m.isEmpty = true → getD m a fallback = fallback :=
   Raw₀.Const.getD_of_isEmpty ⟨m.1, _⟩ m.2
 
-theorem getD_insert [EquivBEq α] [LawfulHashable α] {a k : α} {fallback b : β} :
-    getD (m.insert a b) k fallback = bif a == k then b else getD m k fallback :=
+theorem getD_insert [EquivBEq α] [LawfulHashable α] {k a : α} {fallback v : β} :
+    getD (m.insert k v) a fallback = bif a == k then v else getD m a fallback :=
   Raw₀.Const.getD_insert ⟨m.1, _⟩ m.2
 
 @[simp]
-theorem getD_insert_self [EquivBEq α] [LawfulHashable α] {a : α} {fallback b : β} :
-   getD (m.insert a b) a fallback = b :=
+theorem getD_insert_self [EquivBEq α] [LawfulHashable α] {k : α} {fallback v : β} :
+   getD (m.insert k v) k fallback = v :=
   Raw₀.Const.getD_insert_self ⟨m.1, _⟩ m.2
 
 theorem getD_eq_fallback_of_contains_eq_false [EquivBEq α] [LawfulHashable α] {a : α} {fallback : β} :
@@ -1114,8 +1114,8 @@ theorem getD_eq_fallback [EquivBEq α] [LawfulHashable α] {a : α} {fallback : 
     ¬a ∈ m → getD m a fallback = fallback := by
   simpa [mem_iff_contains] using getD_eq_fallback_of_contains_eq_false
 
-theorem getD_remove [EquivBEq α] [LawfulHashable α] {a k : α} {fallback : β} :
-    getD (m.remove a) k fallback = bif a == k then fallback else getD m k fallback :=
+theorem getD_remove [EquivBEq α] [LawfulHashable α] {k a : α} {fallback : β} :
+    getD (m.remove k) a fallback = bif a == k then fallback else getD m a fallback :=
   Raw₀.Const.getD_remove ⟨m.1, _⟩ m.2
 
 @[simp]
@@ -1154,58 +1154,58 @@ theorem getD_congr [EquivBEq α] [LawfulHashable α] {a b : α} {fallback : β} 
 end Const
 
 @[simp]
-theorem isEmpty_insertIfNew [EquivBEq α] [LawfulHashable α] {a : α} {b : β a} :
-    (m.insertIfNew a b).isEmpty = false :=
+theorem isEmpty_insertIfNew [EquivBEq α] [LawfulHashable α] {k : α} {v : β k} :
+    (m.insertIfNew k v).isEmpty = false :=
   Raw₀.isEmpty_insertIfNew ⟨m.1, _⟩ m.2
 
 @[simp]
-theorem contains_insertIfNew [EquivBEq α] [LawfulHashable α] {a k : α} {b : β a} :
-    (m.insertIfNew a b).contains k = (a == k || m.contains k) :=
+theorem contains_insertIfNew [EquivBEq α] [LawfulHashable α] {k a : α} {v : β k} :
+    (m.insertIfNew k v).contains a = (a == k || m.contains a) :=
   Raw₀.contains_insertIfNew ⟨m.1, _⟩ m.2
 
 @[simp]
-theorem mem_insertIfNew [EquivBEq α] [LawfulHashable α] {a k : α} {b : β a} :
-    k ∈ m.insertIfNew a b ↔ a == k ∨ k ∈ m := by
+theorem mem_insertIfNew [EquivBEq α] [LawfulHashable α] {k a : α} {v : β k} :
+    a ∈ m.insertIfNew k v ↔ a == k ∨ a ∈ m := by
   simp [mem_iff_contains, contains_insertIfNew]
 
 /-- This is a restatement of `contains_insertIfNew` that is written to exactly match the proof obligation in the statement of
     `get_insertIfNew`. -/
-theorem contains_of_contains_insertIfNew [EquivBEq α] [LawfulHashable α] {a k : α} {b : β a} :
-    (m.insertIfNew a b).contains k → ¬((a == k) ∧ m.contains a = false) → m.contains k :=
+theorem contains_of_contains_insertIfNew [EquivBEq α] [LawfulHashable α] {k a : α} {v : β k} :
+    (m.insertIfNew k v).contains a → ¬((a == k) ∧ m.contains k = false) → m.contains a :=
   Raw₀.contains_of_contains_insertIfNew ⟨m.1, _⟩ m.2
 
 /-- This is a restatement of `mem_insertIfNew` that is written to exactly match the proof obligation in the statement of
     `get_insertIfNew`. -/
-theorem mem_of_mem_insertIfNew [EquivBEq α] [LawfulHashable α] {a k : α} {b : β a} :
-    k ∈ m.insertIfNew a b → ¬((a == k) ∧ ¬a ∈ m) → k ∈ m := by
+theorem mem_of_mem_insertIfNew [EquivBEq α] [LawfulHashable α] {k a : α} {v : β k} :
+    a ∈ m.insertIfNew k v → ¬((a == k) ∧ ¬k ∈ m) → a ∈ m := by
   simpa [mem_iff_contains, -contains_insertIfNew] using contains_of_contains_insertIfNew
 
-theorem size_insertIfNew [EquivBEq α] [LawfulHashable α] {a : α} {b : β a} :
-    (m.insertIfNew a b).size = bif m.contains a then m.size else m.size + 1 :=
+theorem size_insertIfNew [EquivBEq α] [LawfulHashable α] {k : α} {v : β k} :
+    (m.insertIfNew k v).size = bif m.contains k then m.size else m.size + 1 :=
   Raw₀.size_insertIfNew ⟨m.1, _⟩ m.2
 
-theorem size_le_size_insertIfNew [EquivBEq α] [LawfulHashable α] {a : α} {b : β a} :
-    m.size ≤ (m.insertIfNew a b).size :=
+theorem size_le_size_insertIfNew [EquivBEq α] [LawfulHashable α] {k : α} {v : β k} :
+    m.size ≤ (m.insertIfNew k v).size :=
   Raw₀.size_le_size_insertIfNew ⟨m.1, _⟩ m.2
 
-theorem get?_insertIfNew [LawfulBEq α] {a k : α} {b : β a} :
-    (m.insertIfNew a b).get? k = if h : a == k ∧ ¬a ∈ m then some (cast (congrArg β (eq_of_beq h.1)) b) else m.get? k := by
+theorem get?_insertIfNew [LawfulBEq α] {k a : α} {v : β k} :
+    (m.insertIfNew k v).get? a = if h : a == k ∧ ¬k ∈ m then some (cast (congrArg β (eq_of_beq h.1).symm) v) else m.get? a := by
   simp only [mem_iff_contains, Bool.not_eq_true]
   exact Raw₀.get?_insertIfNew ⟨m.1, _⟩ m.2
 
-theorem get_insertIfNew [LawfulBEq α] {a k : α} {b : β a} {h₁} :
-    (m.insertIfNew a b).get k h₁ = if h₂ : a == k ∧ ¬a ∈ m then cast (congrArg β (eq_of_beq h₂.1)) b else m.get k
+theorem get_insertIfNew [LawfulBEq α] {k a : α} {v : β k} {h₁} :
+    (m.insertIfNew k v).get a h₁ = if h₂ : a == k ∧ ¬k ∈ m then cast (congrArg β (eq_of_beq h₂.1).symm) v else m.get a
       (mem_of_mem_insertIfNew h₁ h₂) := by
   simp only [mem_iff_contains, Bool.not_eq_true]
   exact Raw₀.get_insertIfNew ⟨m.1, _⟩ m.2
 
-theorem get!_insertIfNew [LawfulBEq α] {a k : α} [Inhabited (β k)] {b : β a} :
-    (m.insertIfNew a b).get! k = if h : a == k ∧ ¬a ∈ m then cast (congrArg β (eq_of_beq h.1)) b else m.get! k := by
+theorem get!_insertIfNew [LawfulBEq α] {k a : α} [Inhabited (β a)] {v : β k} :
+    (m.insertIfNew k v).get! a = if h : a == k ∧ ¬k ∈ m then cast (congrArg β (eq_of_beq h.1).symm) v else m.get! a := by
   simp only [mem_iff_contains, Bool.not_eq_true]
   exact Raw₀.get!_insertIfNew ⟨m.1, _⟩ m.2
 
-theorem getD_insertIfNew [LawfulBEq α] {a k : α} {fallback : β k} {b : β a} :
-    (m.insertIfNew a b).getD k fallback = if h : a == k ∧ ¬a ∈ m then cast (congrArg β (eq_of_beq h.1)) b else m.getD k fallback := by
+theorem getD_insertIfNew [LawfulBEq α] {k a : α} {fallback : β a} {v : β k} :
+    (m.insertIfNew k v).getD a fallback = if h : a == k ∧ ¬k ∈ m then cast (congrArg β (eq_of_beq h.1).symm) v else m.getD a fallback := by
   simp only [mem_iff_contains, Bool.not_eq_true]
   exact Raw₀.getD_insertIfNew ⟨m.1, _⟩ m.2
 
@@ -1213,31 +1213,31 @@ namespace Const
 
 variable {β : Type v} {m : DHashMap α (fun _ => β)}
 
-theorem get?_insertIfNew [EquivBEq α] [LawfulHashable α] {a k : α} {b : β} :
-    get? (m.insertIfNew a b) k = bif a == k && !m.contains a then some b else get? m k :=
+theorem get?_insertIfNew [EquivBEq α] [LawfulHashable α] {k a : α} {v : β} :
+    get? (m.insertIfNew k v) a = bif a == k && !m.contains k then some v else get? m a :=
   Raw₀.Const.get?_insertIfNew ⟨m.1, _⟩ m.2
 
-theorem get_insertIfNew [EquivBEq α] [LawfulHashable α] {a k : α} {b : β} {h₁} :
-    get (m.insertIfNew a b) k h₁ = if h₂ : a == k ∧ ¬a ∈ m then b else get m k (mem_of_mem_insertIfNew h₁ h₂) := by
+theorem get_insertIfNew [EquivBEq α] [LawfulHashable α] {k a : α} {v : β} {h₁} :
+    get (m.insertIfNew k v) a h₁ = if h₂ : a == k ∧ ¬k ∈ m then v else get m a (mem_of_mem_insertIfNew h₁ h₂) := by
   simp only [mem_iff_contains, Bool.not_eq_true]
   exact Raw₀.Const.get_insertIfNew ⟨m.1, _⟩ m.2
 
-theorem get!_insertIfNew [EquivBEq α] [LawfulHashable α] [Inhabited β] {a k : α} {b : β} :
-    get! (m.insertIfNew a b) k = bif a == k && !m.contains a then b else get! m k :=
+theorem get!_insertIfNew [EquivBEq α] [LawfulHashable α] [Inhabited β] {k a : α} {v : β} :
+    get! (m.insertIfNew k v) a = bif a == k && !m.contains k then v else get! m a :=
   Raw₀.Const.get!_insertIfNew ⟨m.1, _⟩ m.2
 
-theorem getD_insertIfNew [EquivBEq α] [LawfulHashable α] {a k : α} {fallback b : β} :
-    getD (m.insertIfNew a b) k fallback = bif a == k && !m.contains a then b else getD m k fallback :=
+theorem getD_insertIfNew [EquivBEq α] [LawfulHashable α] {k a : α} {fallback v : β} :
+    getD (m.insertIfNew k v) a fallback = bif a == k && !m.contains k then v else getD m a fallback :=
   Raw₀.Const.getD_insertIfNew ⟨m.1, _⟩ m.2
 
 end Const
 
 @[simp]
-theorem fst_getThenInsertIfNew? [LawfulBEq α] {a : α} {b : β a} : (m.getThenInsertIfNew? a b).1 = m.insertIfNew a b :=
+theorem fst_getThenInsertIfNew? [LawfulBEq α] {k : α} {v : β k} : (m.getThenInsertIfNew? k v).1 = m.insertIfNew k v :=
   Subtype.eq <| (congrArg Subtype.val (Raw₀.fst_getThenInsertIfNew? _)).trans rfl
 
 @[simp]
-theorem snd_getThenInsertIfNew? [LawfulBEq α] {a : α} {b : β a} : (m.getThenInsertIfNew? a b).2 = m.get? a :=
+theorem snd_getThenInsertIfNew? [LawfulBEq α] {k : α} {v : β k} : (m.getThenInsertIfNew? k v).2 = m.get? k :=
   Raw₀.snd_getThenInsertIfNew? _
 
 namespace Const
@@ -1245,11 +1245,11 @@ namespace Const
 variable {β : Type v} {m : DHashMap α (fun _ => β)}
 
 @[simp]
-theorem fst_getThenInsertIfNew? {a : α} {b : β} : (getThenInsertIfNew? m a b).1 = m.insertIfNew a b :=
+theorem fst_getThenInsertIfNew? {k : α} {v : β} : (getThenInsertIfNew? m k v).1 = m.insertIfNew k v :=
   Subtype.eq <| (congrArg Subtype.val (Raw₀.Const.fst_getThenInsertIfNew? _)).trans rfl
 
 @[simp]
-theorem snd_getThenInsertIfNew? {a : α} {b : β} : (getThenInsertIfNew? m a b).2 = get? m a :=
+theorem snd_getThenInsertIfNew? {k : α} {v : β} : (getThenInsertIfNew? m k v).2 = get? m k :=
   Raw₀.Const.snd_getThenInsertIfNew? _
 
 end Const
