Hashmap/HashMap/Lemmas.lean
@@ -30,7 +30,7 @@ theorem isEmpty_emptyc : (∅ : Raw α β).isEmpty :=
   DHashMap.Raw.isEmpty_emptyc
 
 @[simp]
-theorem isEmpty_insert [EquivBEq α] [LawfulHashable α] {a : α} {b : β} : (m.insert a b).isEmpty = false :=
+theorem isEmpty_insert [EquivBEq α] [LawfulHashable α] {k : α} {v : β} : (m.insert k v).isEmpty = false :=
   DHashMap.Raw.isEmpty_insert h.out
 
 theorem contains_congr [EquivBEq α] [LawfulHashable α] {a b : α} (hab : a == b) : m.contains a = m.contains b :=
@@ -59,27 +59,27 @@ theorem mem_iff_contains {a : α} : a ∈ m ↔ m.contains a :=
   DHashMap.Raw.not_mem_emptyc
 
 @[simp]
-theorem contains_insert [EquivBEq α] [LawfulHashable α] {a k : α} {b : β} : (m.insert a b).contains k = (a == k || m.contains k) :=
+theorem contains_insert [EquivBEq α] [LawfulHashable α] {k a : α} {v : β} : (m.insert k v).contains a = (a == k || m.contains a) :=
   DHashMap.Raw.contains_insert h.out
 
 @[simp]
-theorem mem_insert [EquivBEq α] [LawfulHashable α] {a k : α} {b : β} : k ∈ m.insert a b ↔ a == k ∨ k ∈ m :=
+theorem mem_insert [EquivBEq α] [LawfulHashable α] {k a : α} {v : β} : a ∈ m.insert k v ↔ a == k ∨ a ∈ m :=
   DHashMap.Raw.mem_insert h.out
 
-theorem contains_of_contains_insert [EquivBEq α] [LawfulHashable α] {a k : α} {b : β} :
-    (m.insert a b).contains k → (a == k) = false → m.contains k :=
+theorem contains_of_contains_insert [EquivBEq α] [LawfulHashable α] {k a : α} {v : β} :
+    (m.insert k v).contains a → (a == k) = false → m.contains a :=
   DHashMap.Raw.contains_of_contains_insert h.out
 
-theorem mem_of_mem_insert [EquivBEq α] [LawfulHashable α] {a k : α} {b : β} :
-    k ∈ m.insert a b → (a == k) = false → k ∈ m :=
+theorem mem_of_mem_insert [EquivBEq α] [LawfulHashable α] {k a : α} {v : β} :
+    a ∈ m.insert k v → (a == k) = false → a ∈ m :=
   DHashMap.Raw.mem_of_mem_insert h.out
 
 @[simp]
-theorem contains_insert_self [EquivBEq α] [LawfulHashable α] {a : α} {b : β} : (m.insert a b).contains a :=
+theorem contains_insert_self [EquivBEq α] [LawfulHashable α] {k : α} {v : β} : (m.insert k v).contains k :=
   DHashMap.Raw.contains_insert_self h.out
 
 @[simp]
-theorem mem_insert_self [EquivBEq α] [LawfulHashable α] {a : α} {b : β} : a ∈ m.insert a b :=
+theorem mem_insert_self [EquivBEq α] [LawfulHashable α] {k : α} {v : β} : k ∈ m.insert k v :=
   DHashMap.Raw.mem_insert_self h.out
 
 @[simp]
@@ -93,30 +93,30 @@ theorem size_emptyc : (∅ : Raw α β).size = 0 :=
 theorem isEmpty_eq_size_eq_zero : m.isEmpty = (m.size == 0) :=
   DHashMap.Raw.isEmpty_eq_size_eq_zero
 
-theorem size_insert [EquivBEq α] [LawfulHashable α] {a : α} {b : β} : (m.insert a b).size = bif m.contains a then m.size else m.size + 1 :=
+theorem size_insert [EquivBEq α] [LawfulHashable α] {k : α} {v : β} : (m.insert k v).size = bif m.contains k then m.size else m.size + 1 :=
   DHashMap.Raw.size_insert h.out
 
-theorem size_le_size_insert [EquivBEq α] [LawfulHashable α] {a : α} {b : β} : m.size ≤ (m.insert a b).size :=
+theorem size_le_size_insert [EquivBEq α] [LawfulHashable α] {k : α} {v : β} : m.size ≤ (m.insert k v).size :=
   DHashMap.Raw.size_le_size_insert h.out
 
 @[simp]
-theorem remove_empty {a : α} {c : Nat} : (empty c : Raw α β).remove a = empty c :=
+theorem remove_empty {k : α} {c : Nat} : (empty c : Raw α β).remove k = empty c :=
   ext DHashMap.Raw.remove_empty
 
 @[simp]
-theorem remove_emptyc {a : α} : (∅ : Raw α β).remove a = ∅ :=
+theorem remove_emptyc {k : α} : (∅ : Raw α β).remove k = ∅ :=
   ext DHashMap.Raw.remove_emptyc
 
 @[simp]
-theorem isEmpty_remove [EquivBEq α] [LawfulHashable α] {a : α} : (m.remove a).isEmpty = (m.isEmpty || (m.size == 1 && m.contains a)) :=
+theorem isEmpty_remove [EquivBEq α] [LawfulHashable α] {k : α} : (m.remove k).isEmpty = (m.isEmpty || (m.size == 1 && m.contains k)) :=
   DHashMap.Raw.isEmpty_remove h.out
 
 @[simp]
-theorem contains_remove [EquivBEq α] [LawfulHashable α] {k a : α} : (m.remove k).contains a = (!(k == a) && m.contains a) :=
+theorem contains_remove [EquivBEq α] [LawfulHashable α] {k a : α} : (m.remove k).contains a = (!(a == k) && m.contains a) :=
   DHashMap.Raw.contains_remove h.out
 
 @[simp]
-theorem mem_remove [EquivBEq α] [LawfulHashable α] {k a : α} : a ∈ m.remove k ↔ (k == a) = false ∧ a ∈ m :=
+theorem mem_remove [EquivBEq α] [LawfulHashable α] {k a : α} : a ∈ m.remove k ↔ (a == k) = false ∧ a ∈ m :=
   DHashMap.Raw.mem_remove h.out
 
 theorem contains_of_contains_remove [EquivBEq α] [LawfulHashable α] {k a : α} : (m.remove k).contains a → m.contains a :=
@@ -125,18 +125,18 @@ theorem contains_of_contains_remove [EquivBEq α] [LawfulHashable α] {k a : α}
 theorem mem_of_mem_remove [EquivBEq α] [LawfulHashable α] {k a : α} : a ∈ m.remove k → a ∈ m :=
   DHashMap.Raw.mem_of_mem_remove h.out
 
-theorem size_remove [EquivBEq α] [LawfulHashable α] {a : α} : (m.remove a).size = bif m.contains a then m.size - 1 else m.size :=
+theorem size_remove [EquivBEq α] [LawfulHashable α] {k : α} : (m.remove k).size = bif m.contains k then m.size - 1 else m.size :=
   DHashMap.Raw.size_remove h.out
 
-theorem size_remove_le [EquivBEq α] [LawfulHashable α] {a : α} : (m.remove a).size ≤ m.size :=
+theorem size_remove_le [EquivBEq α] [LawfulHashable α] {k : α} : (m.remove k).size ≤ m.size :=
   DHashMap.Raw.size_remove_le h.out
 
 @[simp]
-theorem fst_containsThenInsert {a : α} {b : β} : (m.containsThenInsert a b).1 = m.insert a b :=
+theorem fst_containsThenInsert {k : α} {v : β} : (m.containsThenInsert k v).1 = m.insert k v :=
   ext (DHashMap.Raw.fst_containsThenInsert h.out)
 
 @[simp]
-theorem snd_containsThenInsert {a : α} {b : β} : (m.containsThenInsert a b).2 = m.contains a :=
+theorem snd_containsThenInsert {k : α} {v : β} : (m.containsThenInsert k v).2 = m.contains k :=
   DHashMap.Raw.snd_containsThenInsert h.out
 
 @[simp]
@@ -150,13 +150,13 @@ theorem getElem?_emptyc {a : α} : (∅ : Raw α β)[a]? = none :=
 theorem getElem?_of_isEmpty [EquivBEq α] [LawfulHashable α] {a : α} : m.isEmpty = true → m[a]? = none :=
   DHashMap.Raw.Const.get?_of_isEmpty h.out
 
-theorem getElem?_insert [EquivBEq α] [LawfulHashable α] {a k : α} {b : β} :
-    (m.insert a b)[k]? = bif a == k then some b else m[k]? :=
+theorem getElem?_insert [EquivBEq α] [LawfulHashable α] {k a : α} {v : β} :
+    (m.insert k v)[a]? = bif a == k then some v else m[a]? :=
   DHashMap.Raw.Const.get?_insert h.out
 
 @[simp]
-theorem getElem?_insert_self [EquivBEq α] [LawfulHashable α] {a : α} {b : β} :
-    (m.insert a b)[a]? = some b :=
+theorem getElem?_insert_self [EquivBEq α] [LawfulHashable α] {k : α} {v : β} :
+    (m.insert k v)[k]? = some v :=
   DHashMap.Raw.Const.get?_insert_self h.out
 
 theorem contains_eq_isSome_getElem? [EquivBEq α] [LawfulHashable α] {a : α} : m.contains a = m[a]?.isSome :=
@@ -168,28 +168,28 @@ theorem getElem?_eq_none_of_contains_eq_false [EquivBEq α] [LawfulHashable α] 
 theorem getElem?_eq_none [EquivBEq α] [LawfulHashable α] {a : α} : ¬a ∈ m → m[a]? = none :=
   DHashMap.Raw.Const.get?_eq_none h.out
 
-theorem getElem?_remove [EquivBEq α] [LawfulHashable α] {a k : α} :
-    (m.remove a)[k]? = bif a == k then none else m[k]? :=
+theorem getElem?_remove [EquivBEq α] [LawfulHashable α] {k a : α} :
+    (m.remove k)[a]? = bif a == k then none else m[a]? :=
   DHashMap.Raw.Const.get?_remove h.out
 
 @[simp]
-theorem getElem?_remove_self [EquivBEq α] [LawfulHashable α] {a : α} : (m.remove a)[a]? = none :=
+theorem getElem?_remove_self [EquivBEq α] [LawfulHashable α] {k : α} : (m.remove k)[k]? = none :=
   DHashMap.Raw.Const.get?_remove_self h.out
 
 theorem getElem?_congr [EquivBEq α] [LawfulHashable α] {a b : α} (hab : a == b) : m[a]? = m[b]? :=
   DHashMap.Raw.Const.get?_congr h.out hab
 
-theorem getElem_insert [EquivBEq α] [LawfulHashable α] {a k : α} {b : β} {h₁} :
-    (m.insert a b)[k]'h₁ = if h₂ : a == k then b else m[k]'(mem_of_mem_insert h h₁ (Bool.eq_false_iff.2 h₂)) :=
+theorem getElem_insert [EquivBEq α] [LawfulHashable α] {k a : α} {v : β} {h₁} :
+    (m.insert k v)[a]'h₁ = if h₂ : a == k then v else m[a]'(mem_of_mem_insert h h₁ (Bool.eq_false_iff.2 h₂)) :=
   DHashMap.Raw.Const.get_insert (h₁ := h₁) h.out
 
 @[simp]
-theorem getElem_insert_self [EquivBEq α] [LawfulHashable α] {a : α} {b : β} :
-    (m.insert a b)[a]'(mem_insert_self h) = b :=
+theorem getElem_insert_self [EquivBEq α] [LawfulHashable α] {k : α} {v : β} :
+    (m.insert k v)[k]'(mem_insert_self h) = v :=
   DHashMap.Raw.Const.get_insert_self h.out
 
-theorem getElem_remove [EquivBEq α] [LawfulHashable α] {a k : α} {h'} :
-    (m.remove a)[k]'h' = m[k]'(mem_of_mem_remove h h') :=
+theorem getElem_remove [EquivBEq α] [LawfulHashable α] {k a : α} {h'} :
+    (m.remove k)[a]'h' = m[a]'(mem_of_mem_remove h h') :=
   DHashMap.Raw.Const.get_remove (h' := h') h.out
 
 theorem getElem?_eq_some_getElem [EquivBEq α] [LawfulHashable α] {a : α} {h' : a ∈ m} : m[a]? = some (m[a]'h') :=
@@ -209,13 +209,13 @@ theorem getElem!_emptyc [Inhabited β] {a : α} : (∅ : Raw α β)[a]! = defaul
 theorem getElem!_of_isEmpty [EquivBEq α] [LawfulHashable α] [Inhabited β] {a : α} : m.isEmpty = true → m[a]! = default :=
   DHashMap.Raw.Const.get!_of_isEmpty h.out
 
-theorem getElem!_insert [EquivBEq α] [LawfulHashable α] [Inhabited β] {a k : α} {b : β} :
-    (m.insert a b)[k]! = bif a == k then b else m[k]! :=
+theorem getElem!_insert [EquivBEq α] [LawfulHashable α] [Inhabited β] {k a : α} {v : β} :
+    (m.insert k v)[a]! = bif a == k then v else m[a]! :=
   DHashMap.Raw.Const.get!_insert h.out
 
 @[simp]
-theorem getElem!_insert_self [EquivBEq α] [LawfulHashable α] [Inhabited β] {a : α} {b : β} :
-    (m.insert a b)[a]! = b :=
+theorem getElem!_insert_self [EquivBEq α] [LawfulHashable α] [Inhabited β] {k : α} {v : β} :
+    (m.insert k v)[k]! = v :=
   DHashMap.Raw.Const.get!_insert_self h.out
 
 theorem getElem!_eq_default_of_contains_eq_false [EquivBEq α] [LawfulHashable α] [Inhabited β] {a : α} :
@@ -226,8 +226,8 @@ theorem getElem!_eq_default [EquivBEq α] [LawfulHashable α] [Inhabited β] {a 
     ¬a ∈ m → m[a]! = default :=
   DHashMap.Raw.Const.get!_eq_default h.out
 
-theorem getElem!_remove [EquivBEq α] [LawfulHashable α] [Inhabited β] {a k : α} :
-    (m.remove a)[k]! = bif a == k then default else m[k]! :=
+theorem getElem!_remove [EquivBEq α] [LawfulHashable α] [Inhabited β] {k a : α} :
+    (m.remove k)[a]! = bif a == k then default else m[a]! :=
   DHashMap.Raw.Const.get!_remove h.out
 
 @[simp]
@@ -266,13 +266,13 @@ theorem getD_emptyc {a : α} {fallback : β} : (∅ : Raw α β).getD a fallback
 theorem getD_of_isEmpty [EquivBEq α] [LawfulHashable α] {a : α} {fallback : β} : m.isEmpty = true → m.getD a fallback = fallback :=
   DHashMap.Raw.Const.getD_of_isEmpty h.out
 
-theorem getD_insert [EquivBEq α] [LawfulHashable α] {a k : α} {fallback b : β} :
-    (m.insert a b).getD k fallback = bif a == k then b else m.getD k fallback :=
+theorem getD_insert [EquivBEq α] [LawfulHashable α] {k a : α} {fallback v : β} :
+    (m.insert k v).getD a fallback = bif a == k then v else m.getD a fallback :=
   DHashMap.Raw.Const.getD_insert h.out
 
 @[simp]
-theorem getD_insert_self [EquivBEq α] [LawfulHashable α] {a : α} {fallback b : β} :
-   (m.insert a b).getD a fallback = b :=
+theorem getD_insert_self [EquivBEq α] [LawfulHashable α] {k : α} {fallback v : β} :
+   (m.insert k v).getD k fallback = v :=
   DHashMap.Raw.Const.getD_insert_self h.out
 
 theorem getD_eq_fallback_of_contains_eq_false [EquivBEq α] [LawfulHashable α] {a : α} {fallback : β} :
@@ -283,8 +283,8 @@ theorem getD_eq_fallback [EquivBEq α] [LawfulHashable α] {a : α} {fallback : 
     ¬a ∈ m → m.getD a fallback = fallback :=
   DHashMap.Raw.Const.getD_eq_fallback h.out
 
-theorem getD_remove [EquivBEq α] [LawfulHashable α] {a k : α} {fallback : β} :
-    (m.remove a).getD k fallback = bif a == k then fallback else m.getD k fallback :=
+theorem getD_remove [EquivBEq α] [LawfulHashable α] {k a : α} {fallback : β} :
+    (m.remove k).getD a fallback = bif a == k then fallback else m.getD a fallback :=
   DHashMap.Raw.Const.getD_remove h.out
 
 @[simp]
@@ -317,62 +317,62 @@ theorem getD_congr [EquivBEq α] [LawfulHashable α] {a b : α} {fallback : β} 
   DHashMap.Raw.Const.getD_congr h.out hab
 
 @[simp]
-theorem isEmpty_insertIfNew [EquivBEq α] [LawfulHashable α] {a : α} {b : β} :
-    (m.insertIfNew a b).isEmpty = false :=
+theorem isEmpty_insertIfNew [EquivBEq α] [LawfulHashable α] {k : α} {v : β} :
+    (m.insertIfNew k v).isEmpty = false :=
   DHashMap.Raw.isEmpty_insertIfNew h.out
 
 @[simp]
-theorem contains_insertIfNew [EquivBEq α] [LawfulHashable α] {a k : α} {b : β} :
-    (m.insertIfNew a b).contains k = (a == k || m.contains k) :=
+theorem contains_insertIfNew [EquivBEq α] [LawfulHashable α] {k a : α} {v : β} :
+    (m.insertIfNew k v).contains a = (a == k || m.contains a) :=
   DHashMap.Raw.contains_insertIfNew h.out
 
 @[simp]
-theorem mem_insertIfNew [EquivBEq α] [LawfulHashable α] {a k : α} {b : β} :
-    k ∈ m.insertIfNew a b ↔ a == k ∨ k ∈ m :=
+theorem mem_insertIfNew [EquivBEq α] [LawfulHashable α] {k a : α} {v : β} :
+    a ∈ m.insertIfNew k v ↔ a == k ∨ a ∈ m :=
   DHashMap.Raw.mem_insertIfNew h.out
 
 /-- This is a restatement of `contains_insertIfNew` that is written to exactly match the proof obligation in the statement of
     `getElem_insertIfNew`. -/
-theorem contains_of_contains_insertIfNew [EquivBEq α] [LawfulHashable α] {a k : α} {b : β} :
-    (m.insertIfNew a b).contains k → ¬((a == k) ∧ m.contains a = false) → m.contains k :=
+theorem contains_of_contains_insertIfNew [EquivBEq α] [LawfulHashable α] {k a : α} {v : β} :
+    (m.insertIfNew k v).contains a → ¬((a == k) ∧ m.contains k = false) → m.contains a :=
   DHashMap.Raw.contains_of_contains_insertIfNew h.out
 
 /-- This is a restatement of `mem_insertIfNew` that is written to exactly match the proof obligation in the statement of
     `getElem_insertIfNew`. -/
-theorem mem_of_mem_insertIfNew [EquivBEq α] [LawfulHashable α] {a k : α} {b : β} :
-    k ∈ m.insertIfNew a b → ¬((a == k) ∧ ¬a ∈ m) → k ∈ m :=
+theorem mem_of_mem_insertIfNew [EquivBEq α] [LawfulHashable α] {k a : α} {v : β} :
+    a ∈ m.insertIfNew k v → ¬((a == k) ∧ ¬k ∈ m) → a ∈ m :=
   DHashMap.Raw.mem_of_mem_insertIfNew h.out
 
-theorem size_insertIfNew [EquivBEq α] [LawfulHashable α] {a : α} {b : β} :
-    (m.insertIfNew a b).size = bif m.contains a then m.size else m.size + 1 :=
+theorem size_insertIfNew [EquivBEq α] [LawfulHashable α] {k : α} {v : β} :
+    (m.insertIfNew k v).size = bif m.contains k then m.size else m.size + 1 :=
   DHashMap.Raw.size_insertIfNew h.out
 
-theorem size_le_size_insertIfNew [EquivBEq α] [LawfulHashable α] {a : α} {b : β} :
-    m.size ≤ (m.insertIfNew a b).size :=
+theorem size_le_size_insertIfNew [EquivBEq α] [LawfulHashable α] {k : α} {v : β} :
+    m.size ≤ (m.insertIfNew k v).size :=
   DHashMap.Raw.size_le_size_insertIfNew h.out
 
-theorem getElem?_insertIfNew [EquivBEq α] [LawfulHashable α] {a k : α} {b : β} :
-    (m.insertIfNew a b)[k]? = bif a == k && !m.contains a then some b else m[k]? :=
+theorem getElem?_insertIfNew [EquivBEq α] [LawfulHashable α] {k a : α} {v : β} :
+    (m.insertIfNew k v)[a]? = bif a == k && !m.contains k then some v else m[a]? :=
   DHashMap.Raw.Const.get?_insertIfNew h.out
 
-theorem getElem_insertIfNew [EquivBEq α] [LawfulHashable α] {a k : α} {b : β} {h₁} :
-    (m.insertIfNew a b)[k]'h₁ = if h₂ : a == k ∧ ¬a ∈ m then b else m[k]'(mem_of_mem_insertIfNew h h₁ h₂) :=
+theorem getElem_insertIfNew [EquivBEq α] [LawfulHashable α] {k a : α} {v : β} {h₁} :
+    (m.insertIfNew k v)[a]'h₁ = if h₂ : a == k ∧ ¬k ∈ m then v else m[a]'(mem_of_mem_insertIfNew h h₁ h₂) :=
   DHashMap.Raw.Const.get_insertIfNew h.out (h₁ := h₁)
 
-theorem getElem!_insertIfNew [EquivBEq α] [LawfulHashable α] [Inhabited β] {a k : α} {b : β} :
-    (m.insertIfNew a b)[k]! = bif a == k && !m.contains a then b else m[k]! :=
+theorem getElem!_insertIfNew [EquivBEq α] [LawfulHashable α] [Inhabited β] {k a : α} {v : β} :
+    (m.insertIfNew k v)[a]! = bif a == k && !m.contains k then v else m[a]! :=
   DHashMap.Raw.Const.get!_insertIfNew h.out
 
-theorem getD_insertIfNew [EquivBEq α] [LawfulHashable α] {a k : α} {fallback b : β} :
-    (m.insertIfNew a b).getD k fallback = bif a == k && !m.contains a then b else m.getD k fallback :=
+theorem getD_insertIfNew [EquivBEq α] [LawfulHashable α] {k a : α} {fallback v : β} :
+    (m.insertIfNew k v).getD a fallback = bif a == k && !m.contains k then v else m.getD a fallback :=
   DHashMap.Raw.Const.getD_insertIfNew h.out
 
 @[simp]
-theorem fst_getThenInsertIfNew? {a : α} {b : β} : (getThenInsertIfNew? m a b).1 = m.insertIfNew a b :=
+theorem fst_getThenInsertIfNew? {k : α} {v : β} : (getThenInsertIfNew? m k v).1 = m.insertIfNew k v :=
   ext (DHashMap.Raw.Const.fst_getThenInsertIfNew? h.out)
 
 @[simp]
-theorem snd_getThenInsertIfNew? {a : α} {b : β} : (getThenInsertIfNew? m a b).2 = get? m a :=
+theorem snd_getThenInsertIfNew? {k : α} {v : β} : (getThenInsertIfNew? m k v).2 = get? m k :=
   DHashMap.Raw.Const.snd_getThenInsertIfNew? h.out
 
 end Raw
@@ -393,7 +393,7 @@ theorem isEmpty_emptyc : (∅ : HashMap α β).isEmpty :=
   DHashMap.isEmpty_emptyc
 
 @[simp]
-theorem isEmpty_insert [EquivBEq α] [LawfulHashable α] {a : α} {b : β} : (m.insert a b).isEmpty = false :=
+theorem isEmpty_insert [EquivBEq α] [LawfulHashable α] {k : α} {v : β} : (m.insert k v).isEmpty = false :=
   DHashMap.isEmpty_insert
 
 theorem contains_congr [EquivBEq α] [LawfulHashable α] {a b : α} (hab : a == b) : m.contains a = m.contains b :=
@@ -422,27 +422,27 @@ theorem mem_iff_contains {a : α} : a ∈ m ↔ m.contains a :=
   DHashMap.not_mem_emptyc
 
 @[simp]
-theorem contains_insert [EquivBEq α] [LawfulHashable α] {a k : α} {b : β} : (m.insert a b).contains k = (a == k || m.contains k) :=
+theorem contains_insert [EquivBEq α] [LawfulHashable α] {k a : α} {v : β} : (m.insert k v).contains a = (a == k || m.contains a) :=
   DHashMap.contains_insert
 
 @[simp]
-theorem mem_insert [EquivBEq α] [LawfulHashable α] {a k : α} {b : β} : k ∈ m.insert a b ↔ a == k ∨ k ∈ m :=
+theorem mem_insert [EquivBEq α] [LawfulHashable α] {k a : α} {v : β} : a ∈ m.insert k v ↔ a == k ∨ a ∈ m :=
   DHashMap.mem_insert
 
-theorem contains_of_contains_insert [EquivBEq α] [LawfulHashable α] {a k : α} {b : β} :
-    (m.insert a b).contains k → (a == k) = false → m.contains k :=
+theorem contains_of_contains_insert [EquivBEq α] [LawfulHashable α] {k a : α} {v : β} :
+    (m.insert k v).contains a → (a == k) = false → m.contains a :=
   DHashMap.contains_of_contains_insert
 
-theorem mem_of_mem_insert [EquivBEq α] [LawfulHashable α] {a k : α} {b : β} :
-    k ∈ m.insert a b → (a == k) = false → k ∈ m :=
+theorem mem_of_mem_insert [EquivBEq α] [LawfulHashable α] {k a : α} {v : β} :
+    a ∈ m.insert k v → (a == k) = false → a ∈ m :=
   DHashMap.mem_of_mem_insert
 
 @[simp]
-theorem contains_insert_self [EquivBEq α] [LawfulHashable α] {a : α} {b : β} : (m.insert a b).contains a :=
+theorem contains_insert_self [EquivBEq α] [LawfulHashable α] {k : α} {v : β} : (m.insert k v).contains k :=
   DHashMap.contains_insert_self
 
 @[simp]
-theorem mem_insert_self [EquivBEq α] [LawfulHashable α] {a : α} {b : β} : a ∈ m.insert a b :=
+theorem mem_insert_self [EquivBEq α] [LawfulHashable α] {k : α} {v : β} : k ∈ m.insert k v :=
   DHashMap.mem_insert_self
 
 @[simp]
@@ -456,10 +456,10 @@ theorem size_emptyc : (∅ : HashMap α β).size = 0 :=
 theorem isEmpty_eq_size_eq_zero : m.isEmpty = (m.size == 0) :=
   DHashMap.isEmpty_eq_size_eq_zero
 
-theorem size_insert [EquivBEq α] [LawfulHashable α] {a : α} {b : β} : (m.insert a b).size = bif m.contains a then m.size else m.size + 1 :=
+theorem size_insert [EquivBEq α] [LawfulHashable α] {k : α} {v : β} : (m.insert k v).size = bif m.contains k then m.size else m.size + 1 :=
   DHashMap.size_insert
 
-theorem size_le_size_insert [EquivBEq α] [LawfulHashable α] {a : α} {b : β} : m.size ≤ (m.insert a b).size :=
+theorem size_le_size_insert [EquivBEq α] [LawfulHashable α] {k : α} {v : β} : m.size ≤ (m.insert k v).size :=
   DHashMap.size_le_size_insert
 
 @[simp]
@@ -471,15 +471,15 @@ theorem remove_emptyc {a : α} : (∅ : HashMap α β).remove a = ∅ :=
   ext DHashMap.remove_emptyc
 
 @[simp]
-theorem isEmpty_remove [EquivBEq α] [LawfulHashable α] {a : α} : (m.remove a).isEmpty = (m.isEmpty || (m.size == 1 && m.contains a)) :=
+theorem isEmpty_remove [EquivBEq α] [LawfulHashable α] {k : α} : (m.remove k).isEmpty = (m.isEmpty || (m.size == 1 && m.contains k)) :=
   DHashMap.isEmpty_remove
 
 @[simp]
-theorem contains_remove [EquivBEq α] [LawfulHashable α] {k a : α} : (m.remove k).contains a = (!(k == a) && m.contains a) :=
+theorem contains_remove [EquivBEq α] [LawfulHashable α] {k a : α} : (m.remove k).contains a = (!(a == k) && m.contains a) :=
   DHashMap.contains_remove
 
 @[simp]
-theorem mem_remove [EquivBEq α] [LawfulHashable α] {k a : α} : a ∈ m.remove k ↔ (k == a) = false ∧ a ∈ m :=
+theorem mem_remove [EquivBEq α] [LawfulHashable α] {k a : α} : a ∈ m.remove k ↔ (a == k) = false ∧ a ∈ m :=
   DHashMap.mem_remove
 
 theorem contains_of_contains_remove [EquivBEq α] [LawfulHashable α] {k a : α} : (m.remove k).contains a → m.contains a :=
@@ -488,18 +488,18 @@ theorem contains_of_contains_remove [EquivBEq α] [LawfulHashable α] {k a : α}
 theorem mem_of_mem_remove [EquivBEq α] [LawfulHashable α] {k a : α} : a ∈ m.remove k → a ∈ m :=
   DHashMap.mem_of_mem_remove
 
-theorem size_remove [EquivBEq α] [LawfulHashable α] {a : α} : (m.remove a).size = bif m.contains a then m.size - 1 else m.size :=
+theorem size_remove [EquivBEq α] [LawfulHashable α] {k : α} : (m.remove k).size = bif m.contains k then m.size - 1 else m.size :=
   DHashMap.size_remove
 
-theorem size_remove_le [EquivBEq α] [LawfulHashable α] {a : α} : (m.remove a).size ≤ m.size :=
+theorem size_remove_le [EquivBEq α] [LawfulHashable α] {k : α} : (m.remove k).size ≤ m.size :=
   DHashMap.size_remove_le
 
 @[simp]
-theorem fst_containsThenInsert {a : α} {b : β} : (m.containsThenInsert a b).1 = m.insert a b :=
+theorem fst_containsThenInsert {k : α} {v : β} : (m.containsThenInsert k v).1 = m.insert k v :=
   ext (DHashMap.fst_containsThenInsert)
 
 @[simp]
-theorem snd_containsThenInsert {a : α} {b : β} : (m.containsThenInsert a b).2 = m.contains a :=
+theorem snd_containsThenInsert {k : α} {v : β} : (m.containsThenInsert k v).2 = m.contains k :=
   DHashMap.snd_containsThenInsert
 
 @[simp]
@@ -513,13 +513,13 @@ theorem getElem?_emptyc {a : α} : (∅ : HashMap α β)[a]? = none :=
 theorem getElem?_of_isEmpty [EquivBEq α] [LawfulHashable α] {a : α} : m.isEmpty = true → m[a]? = none :=
   DHashMap.Const.get?_of_isEmpty
 
-theorem getElem?_insert [EquivBEq α] [LawfulHashable α] {a k : α} {b : β} :
-    (m.insert a b)[k]? = bif a == k then some b else m[k]? :=
+theorem getElem?_insert [EquivBEq α] [LawfulHashable α] {k a : α} {v : β} :
+    (m.insert k v)[a]? = bif a == k then some v else m[a]? :=
   DHashMap.Const.get?_insert
 
 @[simp]
-theorem getElem?_insert_self [EquivBEq α] [LawfulHashable α] {a : α} {b : β} :
-    (m.insert a b)[a]? = some b :=
+theorem getElem?_insert_self [EquivBEq α] [LawfulHashable α] {k : α} {v : β} :
+    (m.insert k v)[k]? = some v :=
   DHashMap.Const.get?_insert_self
 
 theorem contains_eq_isSome_getElem? [EquivBEq α] [LawfulHashable α] {a : α} : m.contains a = m[a]?.isSome :=
@@ -532,28 +532,28 @@ theorem getElem?_eq_none_of_contains_eq_false [EquivBEq α] [LawfulHashable α] 
 theorem getElem?_eq_none [EquivBEq α] [LawfulHashable α] {a : α} : ¬a ∈ m → m[a]? = none :=
   DHashMap.Const.get?_eq_none
 
-theorem getElem?_remove [EquivBEq α] [LawfulHashable α] {a k : α} :
-    (m.remove a)[k]? = bif a == k then none else m[k]? :=
+theorem getElem?_remove [EquivBEq α] [LawfulHashable α] {k a : α} :
+    (m.remove k)[a]? = bif a == k then none else m[a]? :=
   DHashMap.Const.get?_remove
 
 @[simp]
-theorem getElem?_remove_self [EquivBEq α] [LawfulHashable α] {a : α} : (m.remove a)[a]? = none :=
+theorem getElem?_remove_self [EquivBEq α] [LawfulHashable α] {k : α} : (m.remove k)[k]? = none :=
   DHashMap.Const.get?_remove_self
 
 theorem getElem?_congr [EquivBEq α] [LawfulHashable α] {a b : α} (hab : a == b) : m[a]? = m[b]? :=
   DHashMap.Const.get?_congr hab
 
-theorem getElem_insert [EquivBEq α] [LawfulHashable α] {a k : α} {b : β} {h₁} :
-    (m.insert a b)[k]'h₁ = if h₂ : a == k then b else m[k]'(mem_of_mem_insert h₁ (Bool.eq_false_iff.2 h₂)) :=
+theorem getElem_insert [EquivBEq α] [LawfulHashable α] {k a : α} {v : β} {h₁} :
+    (m.insert k v)[a]'h₁ = if h₂ : a == k then v else m[a]'(mem_of_mem_insert h₁ (Bool.eq_false_iff.2 h₂)) :=
   DHashMap.Const.get_insert (h₁ := h₁)
 
 @[simp]
-theorem getElem_insert_self [EquivBEq α] [LawfulHashable α] {a : α} {b : β} :
-    (m.insert a b)[a]'mem_insert_self = b :=
+theorem getElem_insert_self [EquivBEq α] [LawfulHashable α] {k : α} {v : β} :
+    (m.insert k v)[k]'mem_insert_self = v :=
   DHashMap.Const.get_insert_self
 
-theorem getElem_remove [EquivBEq α] [LawfulHashable α] {a k : α} {h'} :
-    (m.remove a)[k]'h' = m[k]'(mem_of_mem_remove h') :=
+theorem getElem_remove [EquivBEq α] [LawfulHashable α] {k a : α} {h'} :
+    (m.remove k)[a]'h' = m[a]'(mem_of_mem_remove h') :=
   DHashMap.Const.get_remove (h' := h')
 
 theorem getElem?_eq_some_getElem [EquivBEq α] [LawfulHashable α] {a : α} {h' : a ∈ m} : m[a]? = some (m[a]'h') :=
@@ -573,13 +573,13 @@ theorem getElem!_emptyc [Inhabited β] {a : α} : (∅ : HashMap α β)[a]! = de
 theorem getElem!_of_isEmpty [EquivBEq α] [LawfulHashable α] [Inhabited β] {a : α} : m.isEmpty = true → m[a]! = default :=
   DHashMap.Const.get!_of_isEmpty
 
-theorem getElem!_insert [EquivBEq α] [LawfulHashable α] [Inhabited β] {a k : α} {b : β} :
-    (m.insert a b)[k]! = bif a == k then b else m[k]! :=
+theorem getElem!_insert [EquivBEq α] [LawfulHashable α] [Inhabited β] {k a : α} {v : β} :
+    (m.insert k v)[a]! = bif a == k then v else m[a]! :=
   DHashMap.Const.get!_insert
 
 @[simp]
-theorem getElem!_insert_self [EquivBEq α] [LawfulHashable α] [Inhabited β] {a : α} {b : β} :
-    (m.insert a b)[a]! = b :=
+theorem getElem!_insert_self [EquivBEq α] [LawfulHashable α] [Inhabited β] {k : α} {v : β} :
+    (m.insert k v)[k]! = v :=
   DHashMap.Const.get!_insert_self
 
 theorem getElem!_eq_default_of_contains_eq_false [EquivBEq α] [LawfulHashable α] [Inhabited β] {a : α} :
@@ -590,8 +590,8 @@ theorem getElem!_eq_default [EquivBEq α] [LawfulHashable α] [Inhabited β] {a 
     ¬a ∈ m → m[a]! = default :=
   DHashMap.Const.get!_eq_default
 
-theorem getElem!_remove [EquivBEq α] [LawfulHashable α] [Inhabited β] {a k : α} :
-    (m.remove a)[k]! = bif a == k then default else m[k]! :=
+theorem getElem!_remove [EquivBEq α] [LawfulHashable α] [Inhabited β] {k a : α} :
+    (m.remove k)[a]! = bif a == k then default else m[a]! :=
   DHashMap.Const.get!_remove
 
 @[simp]
@@ -630,13 +630,13 @@ theorem getD_emptyc {a : α} {fallback : β} : (∅ : HashMap α β).getD a fall
 theorem getD_of_isEmpty [EquivBEq α] [LawfulHashable α] {a : α} {fallback : β} : m.isEmpty = true → m.getD a fallback = fallback :=
   DHashMap.Const.getD_of_isEmpty
 
-theorem getD_insert [EquivBEq α] [LawfulHashable α] {a k : α} {fallback b : β} :
-    (m.insert a b).getD k fallback = bif a == k then b else m.getD k fallback :=
+theorem getD_insert [EquivBEq α] [LawfulHashable α] {k a : α} {fallback v : β} :
+    (m.insert k v).getD a fallback = bif a == k then v else m.getD a fallback :=
   DHashMap.Const.getD_insert
 
 @[simp]
-theorem getD_insert_self [EquivBEq α] [LawfulHashable α] {a : α} {fallback b : β} :
-   (m.insert a b).getD a fallback = b :=
+theorem getD_insert_self [EquivBEq α] [LawfulHashable α] {k : α} {fallback v : β} :
+   (m.insert k v).getD k fallback = v :=
   DHashMap.Const.getD_insert_self
 
 theorem getD_eq_fallback_of_contains_eq_false [EquivBEq α] [LawfulHashable α] {a : α} {fallback : β} :
@@ -647,8 +647,8 @@ theorem getD_eq_fallback [EquivBEq α] [LawfulHashable α] {a : α} {fallback : 
     ¬a ∈ m → m.getD a fallback = fallback :=
   DHashMap.Const.getD_eq_fallback
 
-theorem getD_remove [EquivBEq α] [LawfulHashable α] {a k : α} {fallback : β} :
-    (m.remove a).getD k fallback = bif a == k then fallback else m.getD k fallback :=
+theorem getD_remove [EquivBEq α] [LawfulHashable α] {k a : α} {fallback : β} :
+    (m.remove k).getD a fallback = bif a == k then fallback else m.getD a fallback :=
   DHashMap.Const.getD_remove
 
 @[simp]
@@ -681,62 +681,62 @@ theorem getD_congr [EquivBEq α] [LawfulHashable α] {a b : α} {fallback : β} 
   DHashMap.Const.getD_congr hab
 
 @[simp]
-theorem isEmpty_insertIfNew [EquivBEq α] [LawfulHashable α] {a : α} {b : β} :
-    (m.insertIfNew a b).isEmpty = false :=
+theorem isEmpty_insertIfNew [EquivBEq α] [LawfulHashable α] {k : α} {v : β} :
+    (m.insertIfNew k v).isEmpty = false :=
   DHashMap.isEmpty_insertIfNew
 
 @[simp]
-theorem contains_insertIfNew [EquivBEq α] [LawfulHashable α] {a k : α} {b : β} :
-    (m.insertIfNew a b).contains k = (a == k || m.contains k) :=
+theorem contains_insertIfNew [EquivBEq α] [LawfulHashable α] {k a : α} {v : β} :
+    (m.insertIfNew k v).contains a = (a == k || m.contains a) :=
   DHashMap.contains_insertIfNew
 
 @[simp]
-theorem mem_insertIfNew [EquivBEq α] [LawfulHashable α] {a k : α} {b : β} :
-    k ∈ m.insertIfNew a b ↔ a == k ∨ k ∈ m :=
+theorem mem_insertIfNew [EquivBEq α] [LawfulHashable α] {k a : α} {v : β} :
+    a ∈ m.insertIfNew k v ↔ a == k ∨ a ∈ m :=
   DHashMap.mem_insertIfNew
 
 /-- This is a restatement of `contains_insertIfNew` that is written to exactly match the proof obligation in the statement of
     `getElem_insertIfNew`. -/
-theorem contains_of_contains_insertIfNew [EquivBEq α] [LawfulHashable α] {a k : α} {b : β} :
-    (m.insertIfNew a b).contains k → ¬((a == k) ∧ m.contains a = false) → m.contains k :=
+theorem contains_of_contains_insertIfNew [EquivBEq α] [LawfulHashable α] {k a : α} {v : β} :
+    (m.insertIfNew k v).contains a → ¬((a == k) ∧ m.contains k = false) → m.contains a :=
   DHashMap.contains_of_contains_insertIfNew
 
 /-- This is a restatement of `mem_insertIfNew` that is written to exactly match the proof obligation in the statement of
     `getElem_insertIfNew`. -/
-theorem mem_of_mem_insertIfNew [EquivBEq α] [LawfulHashable α] {a k : α} {b : β} :
-    k ∈ m.insertIfNew a b → ¬((a == k) ∧ ¬a ∈ m) → k ∈ m :=
+theorem mem_of_mem_insertIfNew [EquivBEq α] [LawfulHashable α] {k a : α} {v : β} :
+    a ∈ m.insertIfNew k v → ¬((a == k) ∧ ¬k ∈ m) → a ∈ m :=
   DHashMap.mem_of_mem_insertIfNew
 
-theorem size_insertIfNew [EquivBEq α] [LawfulHashable α] {a : α} {b : β} :
-    (m.insertIfNew a b).size = bif m.contains a then m.size else m.size + 1 :=
+theorem size_insertIfNew [EquivBEq α] [LawfulHashable α] {k : α} {v : β} :
+    (m.insertIfNew k v).size = bif m.contains k then m.size else m.size + 1 :=
   DHashMap.size_insertIfNew
 
-theorem size_le_size_insertIfNew [EquivBEq α] [LawfulHashable α] {a : α} {b : β} :
-    m.size ≤ (m.insertIfNew a b).size :=
+theorem size_le_size_insertIfNew [EquivBEq α] [LawfulHashable α] {k : α} {v : β} :
+    m.size ≤ (m.insertIfNew k v).size :=
   DHashMap.size_le_size_insertIfNew
 
-theorem getElem?_insertIfNew [EquivBEq α] [LawfulHashable α] {a k : α} {b : β} :
-    (m.insertIfNew a b)[k]? = bif a == k && !m.contains a then some b else m[k]? :=
+theorem getElem?_insertIfNew [EquivBEq α] [LawfulHashable α] {k a : α} {v : β} :
+    (m.insertIfNew k v)[a]? = bif a == k && !m.contains k then some v else m[a]? :=
   DHashMap.Const.get?_insertIfNew
 
-theorem getElem_insertIfNew [EquivBEq α] [LawfulHashable α] {a k : α} {b : β} {h₁} :
-    (m.insertIfNew a b)[k]'h₁ = if h₂ : a == k ∧ ¬a ∈ m then b else m[k]'(mem_of_mem_insertIfNew h₁ h₂) :=
+theorem getElem_insertIfNew [EquivBEq α] [LawfulHashable α] {k a : α} {v : β} {h₁} :
+    (m.insertIfNew k v)[a]'h₁ = if h₂ : a == k ∧ ¬k ∈ m then v else m[a]'(mem_of_mem_insertIfNew h₁ h₂) :=
   DHashMap.Const.get_insertIfNew (h₁ := h₁)
 
-theorem getElem!_insertIfNew [EquivBEq α] [LawfulHashable α] [Inhabited β] {a k : α} {b : β} :
-    (m.insertIfNew a b)[k]! = bif a == k && !m.contains a then b else m[k]! :=
+theorem getElem!_insertIfNew [EquivBEq α] [LawfulHashable α] [Inhabited β] {k a : α} {v : β} :
+    (m.insertIfNew k v)[a]! = bif a == k && !m.contains k then v else m[a]! :=
   DHashMap.Const.get!_insertIfNew
 
-theorem getD_insertIfNew [EquivBEq α] [LawfulHashable α] {a k : α} {fallback b : β} :
-    (m.insertIfNew a b).getD k fallback = bif a == k && !m.contains a then b else m.getD k fallback :=
+theorem getD_insertIfNew [EquivBEq α] [LawfulHashable α] {k a : α} {fallback v : β} :
+    (m.insertIfNew k v).getD a fallback = bif a == k && !m.contains k then v else m.getD a fallback :=
   DHashMap.Const.getD_insertIfNew
 
 @[simp]
-theorem fst_getThenInsertIfNew? {a : α} {b : β} : (getThenInsertIfNew? m a b).1 = m.insertIfNew a b :=
+theorem fst_getThenInsertIfNew? {k : α} {v : β} : (getThenInsertIfNew? m k v).1 = m.insertIfNew k v :=
   ext (DHashMap.Const.fst_getThenInsertIfNew?)
 
 @[simp]
-theorem snd_getThenInsertIfNew? {a : α} {b : β} : (getThenInsertIfNew? m a b).2 = get? m a :=
+theorem snd_getThenInsertIfNew? {k : α} {v : β} : (getThenInsertIfNew? m k v).2 = get? m k :=
   DHashMap.Const.snd_getThenInsertIfNew?
 
 instance [EquivBEq α] [LawfulHashable α] : LawfulGetElem (HashMap α β) α β (fun m a => a ∈ m) where
